---
{"dg-publish":true,"permalink":"/MATH/代数专题/Nodes/10 Representation of Symmetric Groups/","dgPassFrontmatter":true}
---



<div class="transclusion internal-embed is-loaded"><a class="markdown-embed-link" href="/math//nodes/10-1-preliminary-for-symmetric-groups/" aria-label="Open link"><svg xmlns="http://www.w3.org/2000/svg" width="24" height="24" viewBox="0 0 24 24" fill="none" stroke="currentColor" stroke-width="2" stroke-linecap="round" stroke-linejoin="round" class="svg-icon lucide-link"><path d="M10 13a5 5 0 0 0 7.54.54l3-3a5 5 0 0 0-7.07-7.07l-1.72 1.71"></path><path d="M14 11a5 5 0 0 0-7.54-.54l-3 3a5 5 0 0 0 7.07 7.07l1.71-1.71"></path></svg></a><div class="markdown-embed">





# Parity and Presentation of Symmetric Groups

> [!definition] parity
> Each permutation in $S_n$ can be presented as a diagram permutation said to be odd (rep. even) if the number of crossing in this diagram is odd (rep. even). Define $\mathrm{sgn}:S_n\to\{\pm1\}$ as $\mathrm{sgn}(\sigma)=1$ if $\sigma$ is even and $\mathrm{sgn}(\sigma)=-1$ if $\sigma$ is odd.
> 
> ![Pasted image 20241104141018.png|300](/img/user/%E9%99%84%E4%BB%B6/Pasted%20image%2020241104141018.png)
> 
> Equivalently, the parity of permutation $\sigma$ is the number of inversions $(i,j)$ in $\sigma$: $1\leqslant i<j\leqslant n$ such that $\sigma(i)<\sigma(j)$.


The adjacent transposition $s_i:=(i\;i+1)$ for all $1\leqslant i\leqslant n-1$, then $S_n$ is generated by $\{s_i:1\leqslant i\leqslant n-1\}$. 


> [!proposition]
> The symmetric group has the following presentation 
> 
> $S_n=\left\langle s_1,\cdots,s_{n-1}: s_i^2=1,s_is_j=s_js_i\mbox{ with }|i-j|>2,s_is_{i+1}s_i=s_{i+1}s_is_{i+1}\right\rangle .$

`\begin{proof}` 
Define the LHS equals $\Gamma_n$. We have a surjective homomorphism $\Gamma_n\to S_n,s_i\mapsto (i\;i+1)$. It suffices to show $|\Gamma_n|\leqslant n!$. Note that the case of $n=1$ holds. Suppose that $|\Gamma_{n}|\leqslant n!$, and consider the subgroup $H<\Gamma_{n+1}$ generated by $s_1,\cdots,s_{n-1}$where $|H|\leqslant n!$ by induction hypothesis. Note that 

$\Gamma_{n+1}=H\cup s_n H\cup\cdots\cup s_1\cdots s_n H$

and this composition is stable by the action of $n$. Therefore, $|\Gamma_{n+1}|\leqslant (n+1)!$ and so $\Gamma_n\simeq S_n$.
`\end{proof}`


> [!definition]
> Any element of $S_n$ can be written as product of $s_i


<div class="transclusion internal-embed is-loaded"><a class="markdown-embed-link" href="/math//nodes/10-2-tableaux-tabloids-and-specht-module/" aria-label="Open link"><svg xmlns="http://www.w3.org/2000/svg" width="24" height="24" viewBox="0 0 24 24" fill="none" stroke="currentColor" stroke-width="2" stroke-linecap="round" stroke-linejoin="round" class="svg-icon lucide-link"><path d="M10 13a5 5 0 0 0 7.54.54l3-3a5 5 0 0 0-7.07-7.07l-1.72 1.71"></path><path d="M14 11a5 5 0 0 0-7.54-.54l-3 3a5 5 0 0 0 7.07 7.07l1.71-1.71"></path></svg></a><div class="markdown-embed">





> [!definition]
> Let $\lambda\vdash n$ be a partition of $n$ with $\lambda=(\lambda_1,\cdots,\lambda_{\ell})$, then define corresponding Young subgroup as
> 
> $S_\lambda=S_{\{1,\cdots,\lambda_1\}}\times\cdots\times S_{\{n-\lambda_\ell,\cdots,n\}}.$

For a trivial representation of $S_\lambda$, we have that 

$\dim\mathrm{tr}\uparrow_{S_\lambda}^{S_n}=\frac{|S_n|}{|S_\lambda|}=\frac{n!}{\lambda _1!\cdots\lambda_{\ell}!}.$

> [!definition] tableau
> Let $\lambda\vdash n$. A Young tableau of shape $\lambda$ is an array obtained by putting $1,\cdots,n$ into $\lambda$-tableau.

For example, see [[Pasted image 20241104154929.png|here]]. Note that $\tau\in S_n$ can naturally act on $\lambda$-tableaus.


> [!definition]
> Two tableaux are equivalent if they are of the same $\lambda$-shape and they have the same element in each row. [[Pasted image 20241104155437.png|Here]] is an example.


> [!definition] tabloid
> Given a tableau $t$, define the tabloid or $\lambda$-tabloid as the set $\{t':t'\sim t\}$.

# the Corresponding Module $M^\lambda$

> [!definition]
> For every partition $\lambda\vdash n$ the corresponding module $M^\lambda$ is the linear space of all tabloids of shape $\lambda$, $M^\lambda\simeq \mathbb{C}[\{t_1\},\cdots.,\{t_n\}]$ where $\dim M^\lambda=\frac{n!}{\lambda!}$ and $\lambda!=\lambda_1!\cdots\lambda_\ell!$.

**Examples.**
- Let $\lambda=(n)$, then $M^{(n)}=\mathbb{C}[\{t\}]$ and $\dim M^{(n)}=1$.
- Let $\lambda=(1,1,\cdots,1)$, then $M^\lambda=\mathbb{C}[\{t_1\},\cdots,\{t_{n!}\}]$ and this action is regular, as $G$ acting on $\mathbb{C}G$. 
- Let $\lambda=(n-1,1)$, then $M^\lambda=\mathbb{C}[\{t_1\},\cdots,\{t_n\}]$ and this action deduces the permutation representation of $S_n$.

> [!proposition]
> Let $\lambda\vdash n$ be a partition, and let $S_\lambda<S_n$ be the subgroup corresponding to $\lambda$. Then $\mathrm{tr}\uparrow_{S_\lambda}^{S_n}\simeq M^\lambda$.

`\begin{proof}`
Define $\varphi:\pi_i \otimes W\mapsto\{\pi_it^\lambda\}$ where $W$ is the trivial $S_\lambda$-module and $t^\lambda$ is the tabloid whose $\ell$ rows are $\{1,\cdots,\lambda_1\}$, $\{\lambda_1+1,\cdots,\lambda_2\}$, ..., $\{n-\lambda_{\ell},\cdots,n\}$. Then $\varphi$ is an isomorphism of $S_n$-modules.
`\end{proof}`


# the Row/Column Stabilizer and the Associated Polytabloid 

> [!definition]
> Let $\lambda\vdash n$ be a partition, and let $t$ be a tableau in $\lambda$-shape. Suppose $t$ has rows $R_1,\cdots,R_\ell$ and columns $C_1,\cdots,C_m$. Define subgroups of $S_n$ as $R_t=S_{R_1}\times\cdots\times S_{R_\ell}$ and $C_t=S_{C_1}\times\cdots\times S_{C_m}$, and they are called the *row-stabilizer* and the *column-stabilizer* of $t$. 

**Remark.** With this definition, we have that $\{t\}=R_t\cdot t$.

> [!definition] associated polytabloid
> For any subset $H\subseteq S_n$, define the following elements of $\mathbb{C}S_n$
> 
> $H^+=\sum_{\pi\in H} \pi,\;H^-=\sum_{\pi\in H}\mathrm{sgn}\pi\cdot \pi=\sum_{\pi\in H}\pi^-,$
> 
> where $\pi^-=\mathrm{sgn}\pi\cdot \pi$. 
> 
> For any tableau $t$ with $C_1,\cdots,C_m$, define 
> 
> $K_{C_i}=C_i^-=\sum_{\pi\in S_{C_i}}\mathrm{sgn}\pi\cdot \pi,\;K_t=K_{c_1}\times\cdots\times K_{C_m}\mbox{ and }e_t=K_t\{t\},$
> 
> where $e_t$ is called the associated polytabloid of $\lambda$-tableau $t$. 

**Remark.** For any $\lambda$-tableau $t$, the associated polytabloid $e_t=K_t\{t\}$ is an element of permutation module $M^\lambda$.

**Example.** Here is an example of $S_5$.

![Pasted image 20241106153505.png|500](/img/user/%E9%99%84%E4%BB%B6/Pasted%20image%2020241106153505.png)


> [!lemma]
> Let $t$ be a tableau and $\sigma\in S_n$. Then:
> - $R_{\sigma t}=\sigma R_t\sigma^{-1}$;
> - $C_{\sigma t}=\sigma C_t\sigma^{-1}$;
> - $K_{\sigma t}=\sigma K_t\sigma^{-1}$;
> - $e_{\sigma t}=\sigma e_t$, where $e$ is the associated polytabloid of $t$. 
`\begin{proof}`
Note that $\pi\in R_{\sigma t}$ iff $\pi\{\sigma t\}=\{\sigma t\}$ iff $\pi\sigma\{t\}=\sigma\{t\}$ iff $\sigma^{-1}t\sigma\{t\}=\{t\}$ iff $\sigma^{-1}t\sigma\in R_t$, and the proof of ii) and iii) are similar. Furthermore, $e_{\sigma t}=K_{\sigma t}\{\sigma t\}=\sigma K_t\sigma^{-1}\{\sigma t\}=\sigma e_t$. 
`\end{proof}`


# Specht Module

> [!definition]
> Let $\lambda\vdash n$. The Specht module $S^\lambda$ is the submodule of $M^\lambda$ spanned by polytabloids $e_t$ where $t$ is of shape $\lambda$.

**Remark.** Since $e_{\sigma t}=\sigma e_t$, any $S^\lambda$ is a cyclic module (a module that is generated by a single element), i.e., it is generated by any tabloid $t$. 

**Examples.** 
- Let $\lambda=(n)$. Then $M^{(n)}=\mathbb{C}[\{t\}]$, $C_t=\{e\}$ and $K_t=e e \cdots e$. Note that $S^\lambda$ is spanned by $e_t=\{t\}$ and $S^\lambda=M^\lambda$.
- Let $\lambda=(1,1,\cdots,1)$. Then $M^{\lambda}=\mathbb{C}[\{t_1\},\cdots,\{t_{n!}\}]$ and $K_t=\sum_{\pi\in S_n}\mathrm{sgn}\pi\cdot \pi$. It follows that $e_t=K_t\{t\}$ and $\sigma e_t=\mathrm{sgn}\sigma\cdot e_t$. Thus, $S^\lambda$ is isomorphic to the sign representation.
- Let $\lambda=(n-1,1)$. Then $M^\lambda=\mathbb{C}[\{t_1\},\cdots,\{t_n\}]$ and $K_t=e-(1n)$. It follows that $e_t=K_t\{t\}=\{t\}-(1n)\{t\}$ and $\sigma e_t=\overline {\mathbf{\sigma(n)}}-\overline {\mathbf{\sigma(1)}}$ where $\overline{\mathbf{k}}$ is the tabloid whose second line is $k$. Thus, $S^\lambda=\{c_1\overline{\mathbf{1}}+\cdots+c_n\overline{\mathbf{n}}:c_1+\cdots+c_n=0\}$ is the standard $S_n$ module.



</div></div>



<div class="transclusion internal-embed is-loaded"><a class="markdown-embed-link" href="/math//nodes/10-3-ordering-of-partitions/" aria-label="Open link"><svg xmlns="http://www.w3.org/2000/svg" width="24" height="24" viewBox="0 0 24 24" fill="none" stroke="currentColor" stroke-width="2" stroke-linecap="round" stroke-linejoin="round" class="svg-icon lucide-link"><path d="M10 13a5 5 0 0 0 7.54.54l3-3a5 5 0 0 0-7.07-7.07l-1.72 1.71"></path><path d="M14 11a5 5 0 0 0-7.54-.54l-3 3a5 5 0 0 0 7.07 7.07l1.71-1.71"></path></svg></a><div class="markdown-embed">





> [!definition] 
> Let $\lambda=(\lambda_1,\cdots,\lambda_\ell)$ and $\mu=(\mu_1,\cdots,\mu_k)$ be $\lambda\vdash n$ and $\mu\vdash n$. Then $\lambda<\mu$ in lexicographic order if for some $i$, $\lambda_j=\mu_j$ for all $j<i$ and $\lambda_i<\mu_i$.  
> [!definition]
> For any $\lambda\vdash n$ and $\mu\vdash n$, if $\lambda_1+\cdots+\lambda_i\leqslant \mu_1+\cdots+\mu_i$ for any $i\geqslant 1$, then we say $\mu$ dominates $\lambda$, written as $\mu\unrhd \lambda$. 

**Example.** Hasse diagram for dominance order for $6$, see [[Pasted image 20241118151234.png|here]].

> [!lemma] dominance lemma
> Let $t$ and $s$ be tableaux of shape $\lambda$ and $\mu$ respectively. If for each index $i$, the elements of row $i$ of $s$ are in different columns in $t$, then $\lambda\unrhd \mu$.  
`\begin{proof}`
We will arrange the tableau $t$ to new form $t'$ by permuting entries within each column. Take elements of the first row of $s$ all in different columns of $t$ and move them to the first row in $t$. Continue to do it for the second row for each $i$. The number of elements in the first $i$ rows of $s$ is $\mu_1+\cdots+\mu_i$ and all elements of first $i$ rows of $\mu$ appears in first $i$ rows of $t'$. Thus for any $i\geqslant 1$, $\lambda_1+\cdots+\lambda_i\geqslant \mu_1+\cdots+\mu_i$ and so $\lambda\unrhd \mu$. As an example, see [[Pasted image 20241118153116.png|here]]. 
`\end{proof}`


</div></div>



<div class="transclusion internal-embed is-loaded"><a class="markdown-embed-link" href="/math//nodes/10-4-complete-list-of-irreducible-modules/" aria-label="Open link"><svg xmlns="http://www.w3.org/2000/svg" width="24" height="24" viewBox="0 0 24 24" fill="none" stroke="currentColor" stroke-width="2" stroke-linecap="round" stroke-linejoin="round" class="svg-icon lucide-link"><path d="M10 13a5 5 0 0 0 7.54.54l3-3a5 5 0 0 0-7.07-7.07l-1.72 1.71"></path><path d="M14 11a5 5 0 0 0-7.54-.54l-3 3a5 5 0 0 0 7.07 7.07l1.71-1.71"></path></svg></a><div class="markdown-embed">





> [!definition]
> For each $M^\lambda=\mathbb{C}[\{t_1\},\cdots,\{t_k\}]$, define an inner product as $\left\langle \{t_i\},\{t_i\}\right\rangle=\delta_{ij}$. Note that this inner produce is $S_n$-invariant, i.e., $\left\langle \pi\{t_i\},\pi\{t_j\}\right\rangle=\left\langle\{t_i\},\{t_j\}\right\rangle$. 

> [!lemma] sign lemma
> Let $H$ be a subgroup of $S_n$.
> - If $\pi\in H$, then $\pi H^-=H^-\pi=(\mathrm{sgn}\pi)H^-$.
> - For any $u,v\in M^\lambda$, $\left\langle H^- u,v\right\rangle=\left\langle u,H^-v\right\rangle$.
> - If $(bc)\in H$, then $H^-=\kappa(1-(bc))$ for some $\kappa\in \mathbb{C}S_n$.
> - If $b$ and $c$ are in the same row of $t$, then $H^-\{t\}=0$. 
`\begin{proof}`
Easy. See [[Pasted image 20241118154911.png|here]].
`\end{proof}`


> [!corollary]
> Let $t$ be tableau of shape $\lambda$ and $s$ be tableau of shape $\mu$, where $\lambda\vdash n$ and $\mu\vdash n$. If $K_t\{s\}\neq 0$, then $\lambda\rhd \mu$. Moreover, if $\lambda=\mu$ and $K_t\{s\}\neq 0$, then $K_t\{s\}=\pm e_t$. 
`\begin{proof}`
Suppose $b$ and $c$ are in the same row of $s$, then they belong to different columns of $t$. Otherwise $K_t\{s\}=\kappa(1-(bc))\{t\}=0$ by [[MATH/代数专题/Nodes/10 Representation of Symmetric Groups#^fae9c5\|#^fae9c5]]. Then by [[MATH/代数专题/Nodes/10.3 Ordering of Partitions#^3e06ba\|10.3 Ordering of Partitions#^3e06ba]] $\lambda\rhd \mu$. If $\lambda=\mu$ and $K_t\{s\}\neq 0$, then $\{s\}=\pi\{t\}$ for some $\pi\in C_t$ (by [[MATH/代数专题/Nodes/10 Representation of Symmetric Groups#^fae9c5\|#^fae9c5]], each pair of numbers in the same column does not appear in the same row of $\{s\}$). It follows that $K_t\{s\}=K_t\{\pi t\}=\mathrm{sgn}\pi K_t\{t\}=\pm e_t$ by [[MATH/代数专题/Nodes/10 Representation of Symmetric Groups#^fae9c5\|#^fae9c5]].
`\end{proof}`


> [!corollary]
> If $u\in M^\mu$ and $t$ is tableau of shape $\mu$, then $K_tu$ is multiple of $e_t$. 

`\begin{proof}`
Since $u$ is a linear combination of tabloid of shape $\mu$, it follows from [[MATH/代数专题/Nodes/10 Representation of Symmetric Groups#^2fe718\|#^2fe718]].
`\end{proof}`


> [!theorem] submodule theorem
> Let $U$ be submodule of $M^\lambda$, then either $U\supseteq S^\lambda$ on or $U\subseteq (S^\lambda)^\bot$. In particular, $S^\lambda$ is irreducible.

`\begin{proof}`
Take $u\in M^\lambda$, then $K_tu=ce_t$ for some $c\in \mathbb{C}$. Suppose that there exists $t$ such that $c\neq 0$. But then $ce_t\in U$. As $S^\lambda$ is cyclic, $\pi(ce_t)$ generates $S^\lambda$ and is inside of $U$, which yields that $S^\lambda\subseteq U$. Otherwise, for any tableau $t$ and $u\in M^\lambda$, we have $K_tu=0$ and so 

$\left\langle u,e_t\right\rangle =\left\langle u,K_t\{t\}\right\rangle =\left\langle K_tu,\{t\}\right\rangle=\left\langle 0,\{t\}\right\rangle =0. $

Therefore, $U\subseteq (S^\lambda)^\bot$. 
`\end{proof}`


> [!proposition]
> If there is a non-zero element $\theta\in \mathrm{Hom}(S^\lambda, M^\mu)$, then $\lambda\rhd \mu$. If $\lambda=\mu$, then $\theta$ is multiplication by a scalar. 
`\begin{proof}`
Since $\theta$ is non-zero, there exists polytabloid $e_t$ such that $\theta(e_t)\neq 0$. Moreover, as $M^\lambda$ can be decomposed as $M^\lambda=S^\lambda\oplus (S^\lambda)^\bot$, we extend $\theta$ to a homomorphism 

$\theta:M^\lambda\to M^\mu,(S^\lambda)^\bot\mapsto 0.$

Since $0\neq \theta(e_t)=\theta(K_t\{t\})=K_t(\theta\{t\})=K_t\sum_i\alpha_i\{s_i\}$ for some $\mu$-tabloids $\{s_i\}$, there is $\lambda\rhd \mu$ by [[MATH/代数专题/Nodes/10 Representation of Symmetric Groups#^2fe718\|#^2fe718]]. 

If $\lambda=\mu$, then $\theta(e_t)=K_t\sum_i\alpha_i\{s_i\}=ce_t$. Then for any permutation $\pi$, 

$\theta(e_{\pi t})=\theta(\pi e_t)=\pi(\theta(e_t))=c\pi e_t=ce_{\pi t}$

and so $\theta$ is a multiplication by $c$.
`\end{proof}`


> [!theorem]
> The Specht modules $S^\lambda$ for $\lambda\vdash \mu$ form a complete list of irreducible modules of $S_n$.

`\begin{proof}`
Since the number of $S^\lambda$ equals the number of $\lambda\vdash n$ and so the number of conjugacy classes of $S_n$, it suffices to show $S^\lambda\neq S^\mu$ for any $\lambda\neq \mu$.

Otherwise, suppose that $S^\lambda =S^\mu$ with $\lambda\neq \mu$. Since $S^\mu\hookrightarrow M^\mu$ is non-trivial, we have non-zero $\theta\in\mathrm{Hom}(S^\lambda, M^\mu)$ and so $\lambda\rhd \mu$ by [[MATH/代数专题/Nodes/10 Representation of Symmetric Groups#^376fda\|#^376fda]]. Similarly we have $\mu\rhd \lambda$ and so $\mu=\lambda$, contradiction. Now we finish the proof.
`\end{proof}`


> [!corollary]
> The irreducible decomposition of the permutation module $M^\lambda$ has the form 
>
> $M^\mu=\oplus_{\lambda\rhd\mu} \kappa_{\lambda\mu}S^\lambda,$
> 
> where $\kappa_{\lambda\mu}$ is called Kostka numbers. Moreover, $\kappa_{\mu\mu}=1$.  
[[Pasted image 20241120154248.png|Here]] is an example.

`\begin{proof}`
Note that $\kappa_{\lambda\mu}=\dim\mathrm{Hom}_{S_n}(S^\lambda,M^\mu)=\left\langle \chi^\lambda,\psi^\mu\right\rangle$ where $\chi^\lambda$ and $\psi^\mu$ are characters of $S^\lambda$ and $M^\mu$, respectively. If $\kappa_{\lambda\mu}\neq 0$, then $\lambda\rhd \mu$ by [[MATH/代数专题/Nodes/10 Representation of Symmetric Groups#^376fda\|#^376fda]]. Furthermore, since $\theta\in \mathrm{Hom}(S^\mu,M^\mu)$ is multiplication by scalar by [[MATH/代数专题/Nodes/10 Representation of Symmetric Groups#^376fda\|#^376fda]], we have $\dim\mathrm{Hom}_{S_n}(S^\lambda,M^\lambda)=\kappa_{\mu\mu}=1$. 
`\end{proof}`




</div></div>



<div class="transclusion internal-embed is-loaded"><a class="markdown-embed-link" href="/math//nodes/10-5-basis-of-specht-modules/" aria-label="Open link"><svg xmlns="http://www.w3.org/2000/svg" width="24" height="24" viewBox="0 0 24 24" fill="none" stroke="currentColor" stroke-width="2" stroke-linecap="round" stroke-linejoin="round" class="svg-icon lucide-link"><path d="M10 13a5 5 0 0 0 7.54.54l3-3a5 5 0 0 0-7.07-7.07l-1.72 1.71"></path><path d="M14 11a5 5 0 0 0-7.54-.54l-3 3a5 5 0 0 0 7.07 7.07l1.71-1.71"></path></svg></a><div class="markdown-embed">





> [!definition]
> A tableau $t$ is called standard if the rows and the columns of $t$ are increasing sequences.  
In this section, we aim to prove the following theorem. The proof is written [[MATH/代数专题/Nodes/10.5 Basis of Specht Modules#^goswcn\|here]]. 

> [!theorem]
> The set $\{e_t:t\mbox{ is a standard }\lambda\mbox{-tableau}\}$ is a basis of Specht module $S^\lambda$.  
We call a sequence $\lambda=(\lambda_1,\cdots,\lambda_k)$ with $\lambda_1+\cdots+\lambda_k=n$ is a composition of $n$, and $\lambda_i$ is called part of $\lambda$. (Compare with partition: composition with $\lambda_1\geqslant \cdots\geqslant\cdots\lambda_k$.) We say that composition $\lambda$ dominates $\mu$, if for any $k\geqslant 1$ there is $\lambda_1+\cdots+\lambda_k\geqslant \mu_1+\cdots+\mu_k$. 

Suppose $\{t\}$ is a tabloid of shape $\lambda\vdash n$. For each $i=1,\cdots,n$, define $\{t^i\}$ as the tabloid formed by all elements $\leqslant i$ in $\{t\}$, and define $\lambda^i$ as the composition which is the shape of $t^i$. Here is an example:

![Pasted image 20241125143011.png|500](/img/user/%E9%99%84%E4%BB%B6/Pasted%20image%2020241125143011.png)

There is a way to order tabloids in the same shape.

> [!definition]
> Let $\{t\}$ and $\{s\}$ be two tabloids in $\lambda$-shape with the corresponding composition $\lambda^i$ and $\mu^i$. We say that $\{s\}$ dominates $\{t\}$, denoted by $\{s\}\rhd\{t\}$ if $\mu^i\rhd \lambda^i$ for all $i$.

**Remark.** Not all tabloids can be compared. For example, take 

$\{t\}=\left\{\
\begin{matrix} 1 & 3 & 4\\
2 & 5  \end{matrix}\right\}\mbox{ and }
\{s\}=\left\{
\begin{matrix} 1 & 2 & 5 \\
3 & 4  \end{matrix}\right\}.$

Note that $\lambda^2=(1,1)\lhd \mu^2=(2,0)$ and $\lambda^4=(3,1)\rhd\mu^4=(2,2)$. 

> [!lemma]
> If $k<\ell$ and $k$ occurs in a lower row than $\ell$ in $\{t\}$, then $\{t\}\lhd(k,\ell)\{t\}$.  
`\begin{proof}`
Let $\lambda^i$ and $\mu^i$ be composition sequences for $\{t\}$ and $(k,\ell)\{t\}$, respectively. If $k\leqslant i\leqslant \ell$, and suppose $\ell$, $k$ is in row $q$, $r$ of $\{t\}$ respectively, then 

$(\lambda^i)_q=(\mu^i)_q-1,(\lambda^i)_r=(\mu^i)_r+1$

and so $\lambda^i\lhd \mu^i$ for all $i$. [[Pasted image 20241128202606.png|Here]] is a illustration.
`\end{proof}`


> [!corollary]
> If $v=\sum_i c_i\{t_i\}\in M^\lambda$, we say that $\{t_i\}$ appears in $v$ if $c_i\neq 0$. If $t$ is a [[MATH/代数专题/Nodes/10.5 Basis of Specht Modules#^8pq74m\|standard tableau]] and $\{s\}$ appears in $e_t$, then $\{t\}\rhd \{s\}$. 

`\begin{proof}`
Write $s=\pi t$ with $\pi\in C_t$. 

We do induction on number of "inversions" in $s$, that is, the number of pairs $(k,\ell)$ such that $k\leqslant \ell$ and $k,\ell$ are in the same column but $k$ is in lower row than $\ell$. Then $\{s\}\lhd (k,\ell) \{s\}$ for each inversion and thus $\{s\}\lhd \{t\}$. Here is an example.

![Pasted image 20241125150516.png|500](/img/user/%E9%99%84%E4%BB%B6/Pasted%20image%2020241125150516.png)

For the last term $\{s\}$, $\{1,2\}$ and $\{3,4\}$ are two inversions. By [[MATH/代数专题/Nodes/10 Representation of Symmetric Groups#^rswrnz\|#^rswrnz]], $\{s\}\lhd (12)\{s\}\lhd (12)(34)\{s\}=\{t\}$.
`\end{proof}`


Now we are ready to prove [[MATH/代数专题/Nodes/10 Representation of Symmetric Groups#^030a4e\|#^030a4e]]. 
`\begin{proof}`
First we prove that they are linear independent. Suppose $c_1e_{t_1}+\cdots+c_ne_{t_n}=0$, and we label $\{t_1\}$ in such way that there is no $i>1$ with $\{t_1\}\rhd \{t_i\}$. Then by corollary $\{t_1\}$ only appears in $e_{t_1}$ and so $c_1=0$. By induction all $c_i=0$, contradiction. 

Next we prove that standard polytabloids of shape $\lambda$ span $S^\lambda$. For a polytabloid $e_t$ with tableau $t$, we may assume that column of $t$ are increasing by replacing $e_t$ with $e_{\sigma t}=\sigma e_t=\mathrm{sgn}(\sigma)e_t$ for some suitable $\sigma\in C_t$. Then if $t$ is not standard, we will find two adjacent elements in one row with $t_{i,j}>t_{i,j+1}$. Now we aim to find a linear combination of polytabloids where this row descent is eliminated. This algorithm uses [Garnir relations](https://en.wikipedia.org/wiki/Garnir_relations), as the following example shows.

> [!note] Example
> Consider the following Young tableau $t$:
> 
> ![Pasted image 20241128213455.png|75](/img/user/%E9%99%84%E4%BB%B6/Pasted%20image%2020241128213455.png)
> 
> There is a row descent in the second row, so we choose the subsets $A$ and $B$ as indicated. 
> 
> Consider all partitions of $A\sqcup B=A_i\sqcup B_i$ with $|A_i|=|A|$ and $|B_i|=|B|$, that is
> 
> $\{5,6\}\sqcup\{2,4\},\{4,6\}\sqcup\{2,5\},\{2,6\}\sqcup\{4,5\},\{4,5\}\sqcup\{2,6\},\{2,5\}\sqcup\{4,6\},\{2,4\}\sqcup\{5,6\},$
> 
> and they corresponds the following polytabloid $t-t_2+t_3+t_4-t_5+t_6$
> 
> ![Pasted image 20241128213634.png|500](/img/user/%E9%99%84%E4%BB%B6/Pasted%20image%2020241128213634.png)
> 
> and the Garnir element $g_{A, B}=1-(45)+(245)+(465)-(2465)+(25)(46)$. One may [[MATH/代数专题/Nodes/10 Representation of Symmetric Groups#^791bdb\|check]] $g_{A,B}e_t=0$ and so 
> 
> $e_t=e_{t_2}-e_{t_3}-e_{t_4}+e_{t_5}-e_{t_6}.$
> 
> Therefore, the row descent in the second row is removed. One can repeatedly apply this procedure to straighten a polytabloid, eventually writing it as a linear combination of standard polytabloids. 

With this example, it suffices to show $g_{A,B}e_t=0$. 

> [!proposition] 
> For a tableau $t$ with a row descent and the corresponding sets $A$ and $B$, we have $g_{A,B}e_t=0$. 
> 
`\begin{proof}`
We claim that $S^-_{A\sqcup B}e_t=\{0\}$. Since $|A|+|B|$ is greater than the size of column containing $A$, for any $\sigma\in C_t$ there exist $a,b\in A\sqcup B$ which are in the same row of $\sigma t$. Then by [[MATH/代数专题/Nodes/10.4 Complete List of Irreducible Modules#^fae9c5\|10.4 Complete List of Irreducible Modules#^fae9c5]], $(ab)\in S_{A\sqcup B}$ yields that $S^-_{A\sqcup B}\{\sigma t\}=\{0\}$. Since $e_t=\sum_{\sigma\in C_t}\mathrm{sgn}\sigma\{\sigma t\}$, there is $S^-_{A\sqcup B}e_t=\{0\}$.

Then consider the coset decomposition of $S_{A\sqcup B}$. Note that 

$S_{A\sqcup B}=\pi_1(S_A\times S_B)\sqcup\cdots\sqcup \pi_\ell(S_A\times S_B)$

where $g_{A,B}=\sum_{k=1}^\ell\mathrm{sgn}\pi_i\cdot \pi_i$. Hence, $S_{A\sqcup B}^-=g_{A,B}(S_A\times S_B)^-$. For any element $\tau\in S_A\times S_B$, $\tau e_t=\mathrm{sgn}\tau\cdot e_t$ and so $(S_A\times S_B)^- e_t=|S_A\times S_B|e_t$. Therefore, 

$\{0\}=S^-_{A\sqcup B}e_t=g_{A,B}(S_A\times S_B)^- e_t=g_{A,B}|S_A\times S_B|e_t$

yields that $g_{A,B}e_t=0$.
`\end{proof}`

Now we finish the proof of [[MATH/代数专题/Nodes/10 Representation of Symmetric Groups#^030a4e\|#^030a4e]]. 
`\end{proof}` 


Now we get a basis of Specht module $S^\lambda$. The corresponding representation of it, is Young natural representation.

Recall that $S_n$ is generated by transpositions $(k\;k+1)$, then we denote $s_k=(k\; k+1)$. For $e_t$ be a polytabloid corresponding to standard tableau, there is
- if $k$ and $k+1$ are in the same column, then $s_ke_t=-e_t$;
- if $k$ and $k+1$ are in the same row, then $(k\;k+1)e_t$ will have row descent and then apply Garnir element;
- if $k$ and $k+1$ are in different columns and different rows, then $(k\; k+1)e_t$ is another polytabloid corresponding to standard tableau.

Therefore, each transposition $(k\;k+1)$ induces a linear transformation on the subspace spanned by s polytabloids corresponding to standard tableaus. We refer to this representation as *Young natural representation*.

**Remark.** Every irreducible representation of $S_n$ has integer values, in particular defined over $\mathbb{R}$. Hence, all representations are of [[MATH/代数专题/Nodes/7 Character Table, Frobenius-Schur Indicator & Complexification#^df16b3\|symmetric type]].

</div></div>



<div class="transclusion internal-embed is-loaded"><a class="markdown-embed-link" href="/math//nodes/10-6-frobenius-character-formula/" aria-label="Open link"><svg xmlns="http://www.w3.org/2000/svg" width="24" height="24" viewBox="0 0 24 24" fill="none" stroke="currentColor" stroke-width="2" stroke-linecap="round" stroke-linejoin="round" class="svg-icon lucide-link"><path d="M10 13a5 5 0 0 0 7.54.54l3-3a5 5 0 0 0-7.07-7.07l-1.72 1.71"></path><path d="M14 11a5 5 0 0 0-7.54-.54l-3 3a5 5 0 0 0 7.07 7.07l1.71-1.71"></path></svg></a><div class="markdown-embed">





> [!theorem] Frobenius character formula
> Let $\lambda\vdash n$ with $\lambda=(\lambda_1,\cdots,\lambda_\ell)$, and let $\lambda_{\ell+1}=\cdots=\lambda_n=0$. The value of $\chi^\lambda$ of $S^\lambda$ on conjugacy class $C_\mu$ given by $\mu=(\mu_1,\cdots,\mu_k)$ with $\mu_1\geqslant\cdots\geqslant \mu_k\geqslant 1$ equals to the coefficient of the monomial $x_1^{\ell_1}\cdots x_n^{\ell_n}$ in polynomial  
> 
> $\prod_{i=1}^k(x_1^{\mu_i}+\cdots+x_n^{\mu_i})\prod_{i<j}(x_i-x_j),$
> 
> where $\ell_i=\lambda_i+n-i$. 

> [!corollary]
> The dimension of Specht module $S^\lambda$ is
> 
> $\dim S^\lambda=f^\lambda=\frac{n!}{\ell_1!\cdots\ell_n!}\prod_{1\leqslant i<j\leqslant n}(\ell_i-\ell_j).$

`\begin{proof}`
Note that $\dim S^\lambda=\chi^\lambda(1)$, then by [[MATH/代数专题/Nodes/10 Representation of Symmetric Groups#^4b468a\|#^4b468a]] 

$\dim S^\lambda=\mbox{ coefficient of }x_1^{\ell_1}\cdots x_n^{\ell_n}\mbox{ in } (x_1+\cdots+x_n)^n\prod_{1\leqslant i<j\leqslant n}(x_i-x_j).$

By Vandermonde determinant, 

$\sum_{\sigma\in S^n}\mathrm{sgn}\sigma \cdot x_1^{n-\sigma(1)}x_2^{n-\sigma(2)-1}\cdots x_n^{n-\sigma(n)}=\det \left|\begin{matrix} x_1^{n-1} & x_2^{n-1} & \cdots & x_n^{n-1} \\
\vdots & \vdots &  & \vdots \\ 
x_1 & x_2 & \cdots & x_n \\
1 & 1 & \cdots & 1\end{matrix}\right|=\prod_{1\leqslant i< j\leqslant n}(x_i-x_j)$

and so the coefficient of $x_1^{\ell_1}\cdots x_n^{\ell_n}$ in

$(x_1+\cdots+x_n)^n\prod_{1\leqslant i<j\leqslant n}(x_i-x_j)=\left(\sum_{k_1+\cdots+k_n=n}\frac{n!}{k_1!\cdots k_n!}x_1^{k_1}\cdots x_n^{k_n}\right)\left(\sum_{\sigma\in S^n}\mathrm{sgn}\sigma \cdot x_1^{n-\sigma(1)}x_2^{n-\sigma(2)-1}\cdots x_n^{n-\sigma(n)}\right)$

is 

$\sum_{\sigma\in S_n}\mathrm{sgn}\sigma\frac{n!}{(\ell_1-n+\sigma(1))!\cdots(\ell_n-n+\sigma(n))!}=n!\det\left|\begin{matrix}
\dfrac{1}{(\ell_1-n+1)!} & \cdots & \dfrac{1}{(\ell_n-n+1)!} \\
\vdots  &  & \vdots \\
\dfrac{1}{\ell_1!} & \cdots & \dfrac{1}{\ell_n!}
\end{matrix}\right|=\frac{n!}{\ell_1!\cdots\ell_n!}\prod_{1\leqslant i<j\leqslant n}(\ell_i-\ell_j).$

Now we finish the proof.
`\end{proof}`


# Hook Length Formula

For a Young tableau $\lambda$ and the element on $i$ th row, $j$ th column, define $h(i,j)=\lambda_i+\lambda_j'-i-j+1$, where $\lambda_j'$ is the number of $j$ th column. 

The hook length formula tells us that

$\dim S^\lambda=f^\lambda=\frac{n!}{\prod_{(i,j)\in\lambda}h(i,j)}.$

[[Pasted image 20241202154117.png|Here]] is an example, and [[MATH/代数专题/Nodes/List 4 (Oral Exam)#^xmv91w\|here]] is a proof.

# Young-Fibonacci Lattice

The number of standard tableaux for $\lambda$ is the number of path from $\emptyset$ to $\lambda$ diagram in Young diagram. Here is an example. 

![Pasted image 20241204154913.png|300](/img/user/%E9%99%84%E4%BB%B6/Pasted%20image%2020241204154913.png). 

</div></div>



<div class="transclusion internal-embed is-loaded"><a class="markdown-embed-link" href="/math//nodes/10-7-branching-rule/" aria-label="Open link"><svg xmlns="http://www.w3.org/2000/svg" width="24" height="24" viewBox="0 0 24 24" fill="none" stroke="currentColor" stroke-width="2" stroke-linecap="round" stroke-linejoin="round" class="svg-icon lucide-link"><path d="M10 13a5 5 0 0 0 7.54.54l3-3a5 5 0 0 0-7.07-7.07l-1.72 1.71"></path><path d="M14 11a5 5 0 0 0-7.54-.54l-3 3a5 5 0 0 0 7.07 7.07l1.71-1.71"></path></svg></a><div class="markdown-embed">





> [!definition]
> A box of $\lambda$ is called removable, if its removal leaves a diagram, which is denoted by $\lambda^-$. 

> [!definition]
> A box of $\lambda$ is called addable to $\lambda$ if the union of $\lambda$ and this box is a diagram.

> [!lemma]
> We have $\dim S^\lambda=f^\lambda=\sum_{\lambda^-}f^{\lambda^-}$.

`\begin{proof}`
Recall that basis of $S^\lambda$ is polytabloids of standard tableaux. Notice every standard tableau consist of $n$ in some removable box and a standard tableau for some $\lambda^-$ and then we finish the proof.
`\end{proof}`


> [!theorem] branching rule
> If $\lambda\vdash n$ is a partition, then 
> 
> $S^\lambda\downarrow_{S_{n-1}}=\oplus_{\lambda^-}S^{\lambda^-}\mbox{ and }S^\lambda\uparrow^{S_{n+1}}=\oplus_{\lambda^+}S^{\lambda^+}.$ 
`\begin{proof}`
Suppose that the removable boxes appear in rows $\tau_1<\cdots<\tau_k$, for each $i$, denote by $\lambda^i$ diagram when you remove box in row $r_i$. For standard tableau $t$ with $n$ in $i$th two denote by $t^i$ tableau obtained by removing box with $n$. Since $S_n$ is a finite group, for any $S_n$-modules $V,W$ with $W\subseteq V$, we have $V\simeq V/W\oplus W$ by [[MATH/Cards/Nodes/Maschke's Theorem\|Maschke's theorem]]. 

To prove the theorem, it suffices to construct chain of $S_{n-1}$-modules

$\{0\}=V^{(0)}\subseteq V^{(1)}\subseteq\cdots\subseteq V^{(k)}=S^\lambda\tag{*}$

such that $V^{(i)}/V^{(i-1)}\simeq S^{\lambda^i}$. 

Define $V^{i}$ as submodule in $S^\lambda$ spanned by all polytabloids corresponding to standard tableaux with $n$ being in the rows $\leqslant i$, that is, $n$ being in rows $r_1,\cdots,r_i$. Then we get $(*)$, the chain of modules what we desire. Define 

$\theta_i:M^\lambda\to M^{\lambda^i},\{t\}\mapsto\begin{cases} \{t^i\} & \mbox{if }n\mbox{ is in the row }r_i\mbox{ of }\{t\}, \\ 0& \mbox{otherwise}. \end{cases}$

Then $\theta_i$ is $S_{n-1}$-homomorphism. Since $n$ occupies a removable box, we have 

$\theta_i:e_t\mapsto\begin{cases} e_{t^i} & \mbox{if }n\mbox{ is in the row }r_i\mbox{ of }\{t\}, \\ 0& \mbox{otherwise}. \end{cases}$

and so $\theta_i V^{(i)}\simeq S^{\lambda^i}$ and $\ker \theta_i=V^{(i-1)}$. It deduces that  

$\dim V^i/V^i\cap \ker \theta_i=\dim\theta_i V^{i}=\dim S^{\lambda^i}=f^{\lambda^i}$

and $(*)$ can be written as 

$\{0\}=V^{(0)}=V^{(1)}\cap \ker\theta_1\subseteq V^{(1)}=V^{(2)}\cap \ker \theta_2\subseteq \cdots\subseteq V^{(k)}=S^\lambda.$

Therefore, we have 

$\sum_{i=1}^k\dim V^{(i)}/V^{(i)}\cap \ker \theta_i=\sum_{i=1}^k f^{\lambda^i}=\dim S^\lambda.$

Furthermore, by [[MATH/代数专题/Nodes/9 Frobenius Reciprocity\|Frobenius reciprocity]], there is 

$m_\mu=\left\langle \chi^\lambda\uparrow ^{S_{n+1}},\chi^\mu\right\rangle=\left\langle \chi^\lambda,\chi^\mu\downarrow_{S_n}\right\rangle=\left\langle \chi^\lambda,\sum_{\mu^-}\chi^{\mu^-}\right\rangle$

and so $m_\mu=0$ if $\lambda\neq \mu^-$ and $m_\mu=1$ if $\lambda=\mu^-$. Note that $\lambda=\mu^-$ iff $\lambda^+=\mu$, thus $\chi^\lambda\uparrow ^{S^{n+1}}=\sum_{\lambda^+}\chi^{\lambda^+}$. Now we finish the proof.
`\end{proof}`


> [!corollary]
> The restriction $S^\lambda\downarrow _{S_{n-1}}$ is irreducible iff the diagram $\lambda=(m^\ell)$, that is, $\lambda$ is a rectangle.



</div></div>



<div class="transclusion internal-embed is-loaded"><a class="markdown-embed-link" href="/math//nodes/10-8-symmetric-polynomials/" aria-label="Open link"><svg xmlns="http://www.w3.org/2000/svg" width="24" height="24" viewBox="0 0 24 24" fill="none" stroke="currentColor" stroke-width="2" stroke-linecap="round" stroke-linejoin="round" class="svg-icon lucide-link"><path d="M10 13a5 5 0 0 0 7.54.54l3-3a5 5 0 0 0-7.07-7.07l-1.72 1.71"></path><path d="M14 11a5 5 0 0 0-7.54-.54l-3 3a5 5 0 0 0 7.07 7.07l1.71-1.71"></path></svg></a><div class="markdown-embed">





# Some Symmetric Polynomials: p, e and h

> [!definition]
> A polynomial in $m$ variables is called *symmetric* if it is stable under all permutations $\sigma\in S_m$, that is, $\sigma(p(x_1,\cdots,x_n))=p(x_{\sigma(1)},\cdots,x_{\sigma(n)})$.
> 
> The algebra of symmetric polynomials is denoted by $\Lambda_m$. 

**Examples.** They are symmetric polynomials.
- $p_n=x_1^n+\cdots+x_m^n$ for all $n\in \mathbb{N}_+$, where the corresponding generated function is $P(t)=\sum_{n=1}^\infty p_nt^{n-1}=\sum_{i=1}^m\dfrac{x_i}{1-x_it}$. 
- The elementary symmetric polynomials $e_n=\sum_{i_1<\cdots<i_n}x_{i_1}\cdots x_{i_n}$ for $n\geqslant 1$. Furthermore, define $e_0=1$. Note that $e_n=0$ when $n\geqslant m$, and the corresponding generated function is $E(t)=\sum_{n=0}^t e_nt^n=\prod_{i=1}^m(1+x_it)$.
- The complete symmetric polynomials $h_n=\sum_{i_1\leqslant\cdots\leqslant i_n}x_{i_1}\cdots x_{i_n}$ for $n\geqslant 1$. We also define $h_0=1$, and the corresponding generated function is $H(t)=\sum_{n=0}^\infty h_nt^n=\prod_{i=1}^\infty\dfrac{1}{1-x_i t}$. 

Since $H(t)E(-t)=1$, we have $\sum_{n=0}^\infty(-1)^re_rh_{n-r}=0$. Next, notice that $p(t)=d/dt\ln\prod_{i=1}^\infty \frac{1}{1-x_it}$, then 

$P(t)=d/dt\ln(H(t))=\frac{H'(t)}{H(t)}.$ 
Similarly $P(-t)=E'(t)/E(t)$. It deduces the Newton identity.

> [!lemma] the Newton identity
> With the definition above, we have $nh_n=\sum_{r=1}^\infty p_rh_{n-r}$ and $ne_n=\sum_{r=1}^n(-1)^{r-1}p_re_{n-r}$.  
> [!proposition]
> If $A$ is an $m \times m$ matrix, then the coefficients of the characteristic polynomial $\operatorname{det}(A-t I)$ are given by the elementary symmetric functions of the eigenvalues $\left\{\lambda_1, \lambda_2, \ldots, \lambda_m\right\}$, with alternating signs $\pm 1$ depending on the degree of each term. The power sums of the eigenvalues coincide with $\operatorname{tr}A^n=\lambda_1^n+\cdots+\lambda_m^n$.

**Remark.** There is some connection between symmetric polynomials and the rooted solution of polynomial equations. See [here](https://math.stackexchange.com/a/96329/1445401). When the degree of polynomial is less than or equal to $4$, the roots can be obtained by operating the coefficients by combination of adding, subtracting, multiplication, division, and taking roots. 

# Schur Polynomial

> [!definition]
> Suppose $\lambda=(\lambda_1,\cdots,\lambda_m)$ is a partition of $n$ of length at most $m$. The Schur polynomial $\mathscr s_\lambda$ is defined by 
> 
> $\mathscr s_\lambda=\frac{\left|\begin{matrix}
x_1^{\lambda_1+m-1} & \cdots  & x_m^{\lambda_1+m-1} \\
x_1^{\lambda_2+m-2} & \cdots & x_m^{\lambda_2+m-2} \\
\vdots &  & \vdots \\
x_1^{\lambda_m} & \cdots & x_m^{\lambda_m}
\end{matrix}\right|}{\left|\begin{matrix}
x_1^{m-1} & \cdots  & x_m^{m-1} \\
x_1^{m-2} & \cdots & x_m^{m-2} \\
\vdots &  & \vdots \\
1 & \cdots & 1
\end{matrix}\right|}.$
> 
> 
For example, when $\lambda=(n)$, $\mathscr s_\lambda=h_n$. When $\lambda=1^n$ and $m=n$, $\mathscr s_\lambda=x_1\cdots x_n$. We can prove them by computing directly, or by the following proposition.

> [!proposition] Jacobi-Trudi formula
> We have 
> 
> $\mathscr s_\lambda=\left|\begin{matrix}h_{\lambda_1} & h_{\lambda_1+1} & \cdots & h_{\lambda_1+m-1} \\ h_{\lambda_2-1} & h_{\lambda_2} & \cdots & h_{\lambda_2+m-2}\\ \vdots & \vdots &  & \vdots \\ h_{\lambda_m-m+1} & h_{\lambda_m-m+2} & \cdots & h_{\lambda_m}\end{matrix}\right|.$ 
`\begin{proof}`
Let $\alpha=(\alpha_1,\cdots,\alpha_m)$ be a composition. Put 

$A_\alpha=\begin{bmatrix} x_1^{\alpha_1} & \cdots & x_m^{\alpha_1} \\
\vdots  &  & \vdots \\
x_1^{\alpha_m} & \cdots & x_m^{\alpha_m} \end{bmatrix}\mbox{ and }H_\alpha =\begin{bmatrix} h_{\alpha_1-m+1} & \cdots & h_{\alpha_1} \\
\vdots  &  & \vdots \\
h_{\alpha_m-m+1} & \cdots & h_{\alpha_m}\end{bmatrix}.$

Consider the elementary symmetric polynomial $e_n^{(k)}$ in variables $x_1,\cdots,\hat x_k,\cdots,x_m$ with $1\leqslant k\leqslant m$ and write them to $m\times m$ matrix 

$M=\begin{bmatrix} (-1)^{m-1}e_{m-1}^{(1)} & \cdots & (-1)^{m-1}e_{m-1}^{(m)} \\
\vdots &  & \vdots \\
(-1)e_1^{(1)} & \cdots & (-1)e_1^{(m)} \\
1 & \cdots & 1\end{bmatrix}.$

We claim that $A_\alpha=H_\alpha M$. Consider generating function for $e_n^{(k)}$ 

$E^{(k)}(t)=\sum_{n=0}^{m-1}e_n^{(k)}t^n=\prod_{i\neq k}(1+x_it),$

then by $H(t)E(-t)=1$ there is 

$H(t)E^{(k)}(t)=\frac{1}{1-x_kt}=1+x_kt+\cdots+(x_kt)^\ell+\cdots.$

Take the coefficient of $t^{\alpha_i}$ and we have 

$\sum_{j=1}^m h_{\alpha_i-m+j}(-1)^{m-j}e_{m-j}^{(k)}=x_k^{\alpha_i}\tag{*}.$

With $(*)$, we can prove the claim. Thus, $\det A_\alpha=\det H_\alpha\det M$ and so $\det H_\alpha=\det A_\alpha/\det M$. For $\delta=(m-1,m-2,\cdots,1,0)$, the matrix $H_\delta=1$ and so $\det A_\delta=\det M$. It follows that 

$\det H_\alpha=\frac{\det A_\alpha}{\det A_\delta}=\mathscr s_\lambda,$

where $\alpha=\lambda+\delta=(\lambda_1+m-1,\lambda_2+m-2,\cdots,\lambda_m)$. Now we finish the proof.
`\end{proof}`


We have a more direct formula for $\mathscr s_\lambda$ by considering a generalized tableau of shape $\lambda$. 


> [!definition] 
> We place numbers $\{1,\cdots,n\}$ into tableau $\lambda\vdash n$ allowing repetition. Such tableau is called *semistandard* if rows are weakly increasing (not decreasing) while columns are strictly increasing sequences. 
> 
> If $T$ is semistandard with $\{1,\cdots,n\}$, set 
> 
> $\mathscr x^T=\prod_{i=1}^n(x_i)^{\operatorname{number of occurrence of }i \in T}.$

> [!proposition]
> For $\lambda\vdash n$ with length $m$, the Schur polynomial in $m$ variables is $\mathscr s_\lambda=\sum_T \mathscr x^T$.

# Basis of $\Lambda_m$

Now we consider algebra of symmetric polynomials in $m$ variables.

First define $\Lambda_m^n=\mathrm{span}\{\mathscr s_\lambda:\lambda\vdash n\}$, the subspace of homogeneous symmetric polynomial of degree $n$, and then define $\Lambda_m=\oplus_{n\geqslant 0}\Lambda_m^n$. 

For example, when $m=3$, we have $\Lambda_m^0=\mathrm{span}\{1\}$, $\Lambda_m^1=\mathrm{span}\{x_1+x_2+x_3\}$,

$\begin{aligned}
\Lambda_m^2&=\mathrm{span}\{\mathscr s_{(1,1)},\mathscr s_{(2,0)}\}=\mathrm{span}\{x_1x_2+x_1x_3+x_2x_3,x_1^2+x_2^2+x_3^2+x_1x_2+x_1x_3+x_2x_3\}, \\
\Lambda_m^3&=\mathrm{span}\{s_{(3)},s_{(2,1)},s_{(1,1,1)}\}=\mathrm{span}\{x_1x_2x_3,x_1^2x_2+x_1^2x_3+x_1x_2^2+2x_1x_2x_3+x_1x_3^2+x_2^2x_3+x_2x_3^2,h_3\}.
\end{aligned}$

> [!proposition]
> $\mathscr s_\lambda$ is a basis for $\Lambda_m$ for all $\lambda\vdash n$ with $n\geqslant 0$. (For a fixed $n$, $\lambda\vdash n$ running through all partitions $\{\mathscr s_\lambda:\lambda\vdash n\}$ is a basis for $\Lambda_m^k$.)

Then we introduce a few families of symmetric polynomials for algebra $\Lambda_m$. 
- For any partition $\lambda=(\lambda_1,\cdots,\lambda_m)$, define $p_\lambda=p_{\lambda_1}\cdots p_{\lambda_m}$, $e_\lambda=e_{\lambda_1}\cdots e_{\lambda_m}$ and $h_\lambda=h_{\lambda_1}\cdots h_{\lambda_m}$. For example, when $m=3$ and $n=2$, $p_{(2)}=p_2=x_1^2+x_2^2+x_3^2$ and $p_{(1,1)}=p_1p_1=(x_1+x_2+x_3)^2$, $e_{(2)}=e_2=x_1x_2+x_2x_3+x_1x_3$ and $e_{(1,1)}=e_1e_1=(x_1+x_2+x_3)^2$, $h_{(2)}=h_2=x_1^2+x_2^2+x_3^2+x_1x_2+x_1x_3+x_2x_3$ and $h_{(1,1)}=h_1h_1=(x_1+x_2+x_3)^2$. 
- Let $\lambda=(\lambda_1,\cdots,\lambda_m)$. Another family of symmetric polynomials is defined as the sum of all different monomials obtained from $x_1^{\lambda_1}\cdots x_m^{\lambda_m}$ under permutation. For example, when $m=3$ and $n=2$, we have $m_{(2)}=x_1^2+x_2^2+x_3^2$, $m_{(1,1)}=2(x_1x_2+x_2x_3+x_1x_3)$. 

> [!theorem]
> Suppose that $\lambda$ runs over all partitions of $n$ of length at most $m$. Then each of the following families is basis of the space $\Lambda_m^n$: 
> 
> $m_\lambda,\mathscr s_\lambda,e_{\lambda'},h_{\lambda'},p_{\lambda'},e_\lambda,h_\lambda,p_\lambda$
> 
> In particular, $\dim \Lambda_m^n=p(n)$ with $m\geqslant n$. 

`\begin{proof}`
We first prove $\{m_\lambda:\lambda\vdash n\}$ is a basis. Note that they are linearly independent: If $\lambda\vdash n$ and $\mu\vdash n$ with $\lambda\neq \mu$, then $m_\lambda$ and $m_\mu$ have no common monomials. Hence, if $\sum_i \alpha_i m_{\lambda_i}=0$, then $\alpha_i=0$. Suppose $f\in \Lambda_m^n$, and we aim to show $f\in\mathrm{span}\{m_\lambda:\lambda\vdash n\}$. We do induction on the order of the element. Take the greatest element $x_1^{n_1}\cdots x_m^{n_m}$ in [[MATH/代数专题/Nodes/10.3 Ordering of Partitions#^0ujtr4\|lexicographic]] order with $\mu=(n_1,\cdots,n_m)$. Then $f-m_\mu\in\Lambda_m^n$ and $f-m_\mu<f$. By induction, $f$ can be written as linear combination of $\{m_\lambda:\lambda\vdash n\}$. 

To show $\mathscr s_\lambda$ form a basis, define $A_m$ as the space of skew-symmetric polynomials in $x_1,\cdots,x_m$. We say $g$ is skew-symmetric if $(ij)g=-g$. It is easy to see that any skew-symmetric polynomials is divisible by $\prod_{1\leqslant i<j\leqslant m}(x_i-x_j)$. We have that $\varphi:\Lambda_m\to A_m,f\mapsto f\prod_{1\leqslant i<j\leqslant m}(x_i-x_j)$, where $\varphi$ defines an isomorphism between $\Lambda_m$ and $A_m$. One can [check](https://math.uchicago.edu/~may/REU2020/REUPapers/Graham.pdf?utm_source=chatgpt.com) that basis of $A_m$ can be given by 

$b_\lambda=\left|\begin{matrix}
x_1^{\lambda_1+m-1} & \cdots & x_m^{\lambda_1+m-1} \\
x_1^{\lambda_2+m-2} & \cdots & x_m^{\lambda_2+m-2} \\
\vdots &  & \vdots \\
x_1^{\lambda_m} & \cdots & x_m^{\lambda_m}
\end{matrix}\right|$

where $\lambda$ runs over through partitions of $n$ of length $\leqslant m$. Notice that $\mathscr s_\lambda=b_\lambda/\prod_{1\leqslant i<j\leqslant m}(x_i-x_j)$ and $\varphi(\mathscr s_\lambda)=b_\lambda$. Furthermore, as $\dim\Lambda_m^n=\dim A_m^{n+{m\choose 2}}$, it deduces that $\mathscr s_\lambda$ form a basis. Moreover, recall that [[MATH/代数专题/Nodes/10.4 Complete List of Irreducible Modules#^i3a31d\|10.4 Complete List of Irreducible Modules#^i3a31d]] and similarly we have $\mathscr s_\mu=\sum_{\lambda}\kappa_{\mu\lambda}m_\lambda=m_\mu+\sum_{\lambda\neq \mu}\kappa_{\mu\lambda}m_\lambda$, and it yields that $\left\langle \mathscr s_\mu:\mu\vdash n\right\rangle=\left\langle m_\mu:\mu\vdash n\right\rangle=\Lambda_m^n$. 

To show $e_{\lambda'}$ form a basis, suppose that $\lambda\vdash n$ with $\lambda=(\lambda_1,\cdots,\lambda_k)$ and $\lambda'=(\rho_1,\cdots,\rho_k)$, and then 

$e_{\lambda'}=e_{\rho_1}\cdots e_{\rho_k}=(x_1\cdots x_{\rho_1}+\cdots)(x_1\cdots x_{\rho_2}+\cdots)\cdots(x_1\cdots x_{\rho_k}+\cdots)=x_1^{\lambda_1}\cdots x_m^{\lambda_m}+\cdots+\mbox{smaller terms}=m_\lambda+\sum_{\mu\lhd\lambda}m_\mu.$

For $h_\lambda$, we can do it by [[MATH/代数专题/Nodes/10 Representation of Symmetric Groups#^jrsjoc\|#^jrsjoc]], as it deduces that $\left\langle \mathscr s_\lambda:\lambda\vdash n\right\rangle\subseteq\left\langle h_\lambda:\lambda\vdash n\right\rangle$. 
`\end{proof}`


> [!definition]
> For each $m$ we have 
> 
> $\Lambda_{m+1}\to \Lambda_m,f(x_1,\cdots,x_m,x_{m+1})\mapsto f(x_1,\cdots,x_m,0)$
> 
> Define a [projective limit](https://en.wikipedia.org/wiki/Inverse_limit) algebra $\Lambda=\oplus_{n\geqslant 0}\Lambda^n$ where $f=(f_m:m\geqslant 0)$ is a sequence of $f_m\in\Lambda_m^n$ and $f_{m+1}\mapsto f_m$ for all $m\geqslant 0$. 

Then $f$ is a formal series in infinitely many variables, and there are several examples:
- $p_n=\sum_{i=1}^\infty x_i^n$
- $e_n=\sum_{1\leqslant i_1<\cdots< i_n}x_{i_1}\cdots x_{i_n}$
- $h_n=\sum_{1\leqslant i_1\leqslant\cdots\leqslant i_n}x_{i_1}\cdots x_{i_n}$

For more details of projective limit, see page 489 of [[Algebra chapter 0 - 2009 - Aluffi.pdf]].
The sequence of Schur polynomials $\mathscr s_\lambda$ defines Schur functions, and the sequence of $m_\lambda$ defines the monomial symmetric functions.

> [!lemma]
> We have
> 
> $h_n=\sum_{\lambda\vdash n}\frac{p_\lambda}{z_\lambda}\mbox{ and }e_n=\sum_{\lambda\vdash n}\frac{\epsilon_\lambda p_\lambda}{z_\lambda}$
> 
> where $\lambda=(1^{m_1},\cdots,n^{m_n})$, $z_\lambda=1^{m_1}m_1! \cdots n^{m_n}m_n!$ and $\epsilon_\lambda=(-1)^{n-\ell(\lambda)}$.


`\begin{proof}`
Recall that 


<div class="transclusion internal-embed is-loaded"><a class="markdown-embed-link" href="/math//nodes/10-8-symmetric-polynomials/#skztji" aria-label="Open link"><svg xmlns="http://www.w3.org/2000/svg" width="24" height="24" viewBox="0 0 24 24" fill="none" stroke="currentColor" stroke-width="2" stroke-linecap="round" stroke-linejoin="round" class="svg-icon lucide-link"><path d="M10 13a5 5 0 0 0 7.54.54l3-3a5 5 0 0 0-7.07-7.07l-1.72 1.71"></path><path d="M14 11a5 5 0 0 0-7.54-.54l-3 3a5 5 0 0 0 7.07 7.07l1.71-1.71"></path></svg></a><div class="markdown-embed">



$P(t)=d/dt\ln(H(t))=\frac{H'(t)}{H(t)}.$ 

</div></div>


It follows 

$H(t)=\exp(\sum_{k=1}^\infty \frac{p_kt^k}{k})=\prod_{k=1}^\infty\exp(\frac{p_kt^k}{k})=\left( 1+p_1t+\frac{(p_1t)^2}{2!}+\cdots\right)\left( 1+\frac{p_2t}{2}+\frac{(p_1t)^2}{2^2\cdot2!}+\cdots\right)\left( 1+\frac{p_3t}{3}+\frac{(p_3t)^2}{3^2\cdot 2!}+\cdots\right)$

and it deduces what we desire. Similarly we can prove $e_n=\sum_{\lambda\vdash n}{\epsilon_\lambda p_\lambda}/{z_\lambda}$.
`\end{proof}`


> [!proposition] orthogonal properties
> For two families of variables $x=(x_1,\cdots,x_k,\cdots)$ and $y=(y_1,\cdots,y_k,\cdots)$, we have the following properties
> 
> $\begin{aligned}
> \prod_{i,j\geqslant 1}(1-x_iy_j)^{-1}&=\sum_{\lambda}z_\lambda^{-1}p_\lambda(x)p_\lambda(y),\\
> \prod_{i,j\geqslant 1}(1-x_iy_j)^{-1}&=\sum_\lambda h_\lambda(x)m_\lambda(y)=\sum_\lambda m_\lambda(x)h_\lambda(y)=\sum_\lambda \mathscr s_\lambda(x)\mathscr s_\lambda(y).
> \end{aligned}$
> 

`\begin{proof}`
By [[MATH/代数专题/Nodes/10 Representation of Symmetric Groups#^dbe3dc\|#^dbe3dc]], we have

$\prod_{i\geqslant 1}(1-x_it)^{-1}=\sum_\lambda z_\lambda^{-1}p_\lambda t^{|\lambda|}\tag{*}$

where $|\lambda|$ is the length of $\lambda$. 

Note that $\sum_{i,j}(x_iy_j)^k=p_k(x)p_k(y)$. Use $(*)$ for $x_iy_j$ and set $t=1$, we have 

$\prod_{i,j\geqslant 1}(1-x_i y_j)^{-1}=\sum_\lambda z_\lambda^{-1} p_\lambda(x_iy_j)=\sum_\lambda z_\lambda^{-1}p_\lambda(x_i)p_\lambda(y_j).$

Equip $\Lambda$ with the following form $\left\langle h_\lambda, m_\mu\right\rangle=\delta_{\lambda\mu}$, and it deduces that $\left\langle p_\lambda,p_\mu\right\rangle=z_\lambda \delta_{\lambda\mu}$ and $\left\langle \mathscr s_\lambda,\mathscr s_\mu\right\rangle=\delta_{\lambda\mu}$. With respect to this inner product, $\{\mathscr s_\lambda:\lambda\vdash n\}$ is orthonormal basis of $\Lambda^n$. 
`\end{proof}`




</div></div>



<div class="transclusion internal-embed is-loaded"><a class="markdown-embed-link" href="/math//nodes/10-9-characteristical-map/" aria-label="Open link"><svg xmlns="http://www.w3.org/2000/svg" width="24" height="24" viewBox="0 0 24 24" fill="none" stroke="currentColor" stroke-width="2" stroke-linecap="round" stroke-linejoin="round" class="svg-icon lucide-link"><path d="M10 13a5 5 0 0 0 7.54.54l3-3a5 5 0 0 0-7.07-7.07l-1.72 1.71"></path><path d="M14 11a5 5 0 0 0-7.54-.54l-3 3a5 5 0 0 0 7.07 7.07l1.71-1.71"></path></svg></a><div class="markdown-embed">





For a finite group $G$, its irreducible characters form basis for the space of class functions $F_c(G,\mathbb{C})$. Define $R_n=F_c(S_n,\mathbb{C})$ and $R=\oplus_{n\geqslant 0}R_n$ with $R_0=\mathbb{C}$. 

We introduce on the $R$ product. For any $\phi\in R_n$ and $\psi\in R_m$, where $\phi$ (rep. $\psi$) is a character of $S_n$ (rep. $S_m$), define $\phi\cdot\psi\in R_{n+m}$ as 

$\phi\cdot \psi=(\phi\otimes \psi)\uparrow_{Sn\times S_m}^{S_{n+m}}.$

> [!theorem]
> The product $\cdot$ on $R$ is commutative and associative.

`\begin{proof}`
Define $\rho=\left(\begin{array}{ccc}1 & \cdots & n & n+1 & \cdots & m\\ m+1& \cdots & n+m & 1 & \cdots & m\end{array}\right)$. Then there is a bijection 

$S_n\times S_m\to S_m\times S_n,\omega\mapsto \rho^{-1}\omega\rho.$

For associativity, use $\left(W\uparrow_K ^H\right)\uparrow_H^G=W \uparrow_K^G$.
`\end{proof}`


Furthermore, we can equip the algebra $R$ with an inner product

$
\left\langle f, g\right\rangle=\sum_{n \geqslant 0}\left\langle f_n,g_n\right\rangle _{S_n}.
$

> [!definition]
> Define the character map 
> 
> $\mathrm{ch}:R\to \Lambda,f\mapsto \frac{1}{n!}\sum_{\omega\in S_n}f(\omega)p_\omega.$
> 

**Remark.** For any $f\in R_n$ and any conjugacy class $C_\mathscr p$ with representative $\mathscr p$, we can write the character map as

$\mathrm{ch}:f\to \frac{1}{n!}\sum_{\mathscr p\vdash n}f(C_p)p_{\mathscr p}|C_{\mathscr p}|=\sum_{\mathscr p\vdash n}z_{\mathcal p}^{-1}f(C_\mathscr p)p_\mathscr p.$

> [!theorem]
> The characteristic map $\mathrm{ch}:R\to \Lambda$ is an isometry and an algebra isomorphism. Moreover, $\mathrm{ch}(\chi^\lambda)=\mathscr s_\lambda$ and $\mathrm{ch}(\phi^\lambda)=h_{\lambda}$, where $\phi^\lambda$ is the character of permutation module $M^\lambda$. 
`\begin{proof}`

> [!NOTE] A Generalization
> Let $G$ be a finite group, and let $A$ be an associative algebra. If $\Phi,\Psi:G\to A$ are functions, we may define a bilinear form with values in $A$ 
> 
> $\left\langle\Phi,\Psi\right\rangle =\frac{1}{|G|}\sum_{g\in G}\Phi(g)\Psi(g^{-1}).$
> 
> If $\Phi$ is a class function on $H$ and $\Psi$ is a class function on $G$, the generalized [[MATH/代数专题/Nodes/9 Frobenius Reciprocity\|Frobenius reciprocity]] still holds, that is 
> 
> $\left\langle \Phi\uparrow^G,\Psi\right\rangle =\left\langle \Phi,\Psi\downarrow_H\right\rangle$
> 
> where $\Phi\downarrow_H(h)=\Phi(h)$ and $\Psi\uparrow ^G(g)=\frac{1}{|H|}\sum_{x\in G}\Psi(x^{-1}gx)$ with the convention that $\Psi(g')=0$ if $g'\notin H$. 

For any $f,g\in R_n$, there is

$\begin{aligned}
\left\langle \mathrm{ch}(f),\mathrm{ch}(g)\right\rangle &=\left\langle \sum_{\mathscr p\vdash n}z_{\mathscr p}^{-1}f(C_{\mathscr p})p_{\mathscr p},\sum_{\lambda\vdash n}z_{\lambda}^{-1}g(C_\lambda)p_\lambda\right\rangle \\
&=\sum_{\lambda\vdash n}z_{\lambda}^{-1}z_{\lambda}^{-1}f(C_\lambda)g(C_\lambda)z_{\lambda}\\
&=\sum_{\lambda\vdash n}|C_\lambda|\frac{1}{n!}f(C_\lambda)g(C_\lambda)\\
&=\left\langle f,g\right\rangle 
\end{aligned}$

Also note that $g(\omega^{-1})=g(\omega)$. 

Since $p_\omega=p_{\omega^{-1}}$ for $\omega\in S_n$ and $\mathrm{ch}(f)=\left\langle f,p\right\rangle$, we have

$\begin{aligned}
\mathrm{ch}(fg)&=\left\langle fg,p\right\rangle=\left\langle(f\otimes g)\uparrow_{S_n\times S_m}^{S_{m\times n}},p\right\rangle\\
&=\frac{1}{n!m!}\sum_{\sigma\in S_n,\tau\in S_m}(f\otimes g)(\sigma\tau)p_{\sigma\tau}\\
&=\frac{1}{n!m!}\sum_{(\sigma,\tau)\in S_n\times S_m}f(\sigma)g(\tau)p_\sigma p_\tau\\
&=\left(\frac{1}{n!}\sum_{\sigma\in S_n}f(\sigma)p_\sigma\right)\left(\frac{1}{m!}\sum_{\tau\in S_m}g(\tau)p_\tau\right)\\
&=\mathrm{ch}(f)\mathrm{ch}(g)
\end{aligned}$

and so $\mathrm{ch}$ is a homomorphism.

Let $\eta_n$ be the trivial representation of $S_n$, then 

$\mathrm{ch}(\eta_n)=\left\langle \eta_n,p\right\rangle=\sum_{\lambda\vdash n}z_{\lambda}^{-1}p_\lambda=h_\lambda.$

Recall that the permutation module $M^\lambda=1\uparrow_{S_\lambda}^{S_n}$ with $S_\lambda=S_{\lambda_1}\times\cdots\times S_{\lambda_k}$. Then $\phi^\lambda=\eta_{\lambda_1}\cdots\eta_{\lambda_k}$ yields that 

$\mathrm{ch}(\phi^\lambda)=\mathrm{ch}(\eta_{\lambda_1})\cdots\mathrm{ch}(\eta_{\lambda_k})=h_{\lambda_1}\cdots h_{\lambda_k}=h_\lambda.$

To prove that $\mathrm{ch}(\chi^\lambda)=\mathscr s_\lambda$, note that

$\widetilde {\chi^\lambda}=\left|\begin{matrix}
\eta_{\lambda_1} & \cdots & \eta_{\lambda_1+m-1} \\
\vdots &  & \vdots \\
\eta_{\lambda_m-m+1} & \cdots & \eta_{\lambda_m}
\end{matrix}\right|$

and $\mathrm{ch}(\widetilde {\chi^\lambda})=\mathscr s_\lambda$. Now we finish the proof, as $\widetilde {\chi^\lambda}$ is induced $\chi^\lambda$. 
`\end{proof}`


> [!corollary]
> The character table $\chi_{\mathscr p}^\lambda$ is the transition matrix between bases $p_\lambda$ and $\mathscr s_\lambda$ of $\Lambda^n$.


`\begin{proof}`
It suffices to show $p_{\mathscr p}=\sum_{\lambda}\chi_{\mathscr p}^\lambda \mathscr s_\lambda$. By [[MATH/代数专题/Nodes/10 Representation of Symmetric Groups#^492b55\|#^492b55]] we have 

$\mathscr s_\lambda=\mathrm{ch}(\chi^\lambda)=\sum_{\mathscr p}z_{\mathscr p}^{-1}\chi_{\mathscr p}^\lambda p_{\mathscr p}$

and so $\chi_{\mathscr p}^\lambda=\left\langle \mathscr s_\lambda, p_\mathscr p\right\rangle$. It deduces that 

$\left\langle \mathscr s_\lambda,p_\mu\right\rangle =\sum_{\mathscr p} z_\mathscr p^{-1}\chi_{\mathscr p}^{\lambda}\left\langle p_\mathscr p,p_\mu\right\rangle =z_{\mu}^{-1}\chi_{\mu}^\lambda z_{\mu}=\chi_{\mu}^\lambda.$

Now we finish the proof.
`\end{proof}`


> [!corollary] Frobenius character formula 
> If $\rho=(\rho_1,\cdots,\rho_m)$ with $\rho_1\geqslant \rho_2\geqslant\cdots\geqslant \rho_m\geqslant 1$, then for any $k\geqslant\ell(\lambda)$ the value $\chi_\rho^\lambda$ is the coefficient of $x_1^{\ell_1}\cdots x_k^{\ell_k}$ in the monomial 
> 
> $\prod_{i=1}^m(x_1^{\rho_i}+\cdots+x_k^{\rho_i})\prod_{1\leqslant i< j\leqslant k}(x_i-x_j)$
> 
> where $\ell_i=\lambda_i+k-i$ for $i=1,\cdots,k$. 

**Remark.** It has been proved in [[MATH/代数专题/Nodes/10.6 Frobenius Character Formula#^4b468a\|10.6 Frobenius Character Formula#^4b468a]].

`\begin{proof}`
Recall that $p_{\rho}=\prod_{i=1}^m(x_1^{\rho_i}+\cdots+x_k^{\rho_i})$ and 


<div class="transclusion internal-embed is-loaded"><a class="markdown-embed-link" href="/math//nodes/10-8-symmetric-polynomials/#i6y60w" aria-label="Open link"><svg xmlns="http://www.w3.org/2000/svg" width="24" height="24" viewBox="0 0 24 24" fill="none" stroke="currentColor" stroke-width="2" stroke-linecap="round" stroke-linejoin="round" class="svg-icon lucide-link"><path d="M10 13a5 5 0 0 0 7.54.54l3-3a5 5 0 0 0-7.07-7.07l-1.72 1.71"></path><path d="M14 11a5 5 0 0 0-7.54-.54l-3 3a5 5 0 0 0 7.07 7.07l1.71-1.71"></path></svg></a><div class="markdown-embed">



> [!definition]
> Suppose $\lambda=(\lambda_1,\cdots,\lambda_m)$ is a partition of $n$ of length at most $m$. The Schur polynomial $\mathscr s_\lambda$ is defined by 
> 
> $\mathscr s_\lambda=\frac{\left|\begin{matrix}
x_1^{\lambda_1+m-1} & \cdots  & x_m^{\lambda_1+m-1} \\
x_1^{\lambda_2+m-2} & \cdots & x_m^{\lambda_2+m-2} \\
\vdots &  & \vdots \\
x_1^{\lambda_m} & \cdots & x_m^{\lambda_m}
\end{matrix}\right|}{\left|\begin{matrix}
x_1^{m-1} & \cdots  & x_m^{m-1} \\
x_1^{m-2} & \cdots & x_m^{m-2} \\
\vdots &  & \vdots \\
1 & \cdots & 1
\end{matrix}\right|}.$
> 
> 

</div></div>


By [[MATH/代数专题/Nodes/10 Representation of Symmetric Groups#^7ed3d1\|#^7ed3d1]], we have $p_{\mathscr p}=\sum_{\lambda}\chi_{\mathscr p}^\lambda \mathscr s_\lambda$ and it deduces that 

$\mathrm{LHS}=\sum_{\mu}\chi_{\rho}^\mu\left|\begin{matrix}
x_1^{\mu_1+k-1} & ... & x_k^{\mu_1+k-1} \\
\vdots &  & \vdots \\
x_1^{\mu_l} & \cdots & x_k^{\mu_k}
\end{matrix}\right|.$

Therefore, the coefficient of $x_1^{\ell_1}\cdots x_k^{\ell_k}$ with $\ell_i=\lambda_i+k-i$ of right hand side is $\chi_{\rho}^\lambda$. 
`\end{proof}`

</div></div>

s, and for $\sigma=s_{i_1}\cdots s_{i_\ell}$, then minimum value of $\ell$ is called the length of $\sigma$.


# Cycle Types and Partitions

> [!definition]
> Any permutation $\sigma$ can be written as product of disjoint cycles. The cycle type is the set of length of cycles. For example, the cycle type of $(1234)(567)$ in $S_8$ is $\{1,3,4\}$. 
> 
> As two permutations with the same cycle type belong to the same conjugacy class, the conjugacy classes of $S_n$ can be described  as $\lambda=(\lambda_1,\cdots,\lambda_\ell)$ with $\lambda_i>0,\lambda_i\in \mathbb{Z}$ and $\lambda_1+\cdots+\lambda_{\ell}=n$.

[[399941730704320_.pic.jpg|There]] are some properties of [partition functions](https://en.wikipedia.org/wiki/Partition_function_(number_theory)). Write partition in the multiplicity from $\lambda=\{1^{m_1},\cdots,n^{m_n}\}$ with $n=m_1+2m_2+\cdots+nm_n$, then we have the following property.

> [!proposition]
> The cardinality of conjugacy class $C_\lambda$ of $S_n$ corresponding to partition $\lambda=\{1^{m_1},\cdots, n^{m_n}\}$ is 
> 
> $|C_\lambda|=\frac{n!}{1^{m_1}m_1!\cdots n^{m_n}m_n!}.$

`\begin{proof}`
Note that 
- $(123),(231),(312)$ are same cycles and there are $1^{m_1}\cdots n^{m_n}$ repetitions.
- $(123)(456)$ and $(456)(123)$ are same cycles and there are $m_1!\cdots m_n!$ repetitions.

Now we finish the proof.
`\end{proof}`

For any given $n\in \mathbb{N}_+$, define $p(n)$ as the number of partitions of $n$. Then we can get its generating function.


> [!theorem] Euler formula
> The generating function for partition is 
> 
> $\sum_{n\geqslant 0}p(n)t^n=\frac{1}{1-t}\frac{1}{1-t^2}\cdots\frac{1}{1-t^n}\cdots$
> 
> where $p(n)$ is the number of partitions of $n$.






</div></div>


![[MATH/代数专题/Nodes/10.2 Tableaux, Tabloids and Specht Module\|10.2 Tableaux, Tabloids and Specht Module]]

![[MATH/代数专题/Nodes/10.3 Ordering of Partitions\|10.3 Ordering of Partitions]]

![[MATH/代数专题/Nodes/10.4 Complete List of Irreducible Modules\|10.4 Complete List of Irreducible Modules]]

![[MATH/代数专题/Nodes/10.5 Basis of Specht Modules\|10.5 Basis of Specht Modules]]

![[MATH/代数专题/Nodes/10.6 Frobenius Character Formula\|10.6 Frobenius Character Formula]]

![[MATH/代数专题/Nodes/10.7 Branching Rule\|10.7 Branching Rule]]

![[MATH/代数专题/Nodes/10.8 Symmetric Polynomials\|10.8 Symmetric Polynomials]]

![[MATH/代数专题/Nodes/10.9 Characteristical Map\|10.9 Characteristical Map]]
