---
{"dg-publish":true,"permalink":"/MATH/代数专题/Nodes/10.6 Frobenius Character Formula/","dgPassFrontmatter":true}
---


> [!theorem] Frobenius character formula
> Let $\lambda\vdash n$ with $\lambda=(\lambda_1,\cdots,\lambda_\ell)$, and let $\lambda_{\ell+1}=\cdots=\lambda_n=0$. The value of $\chi^\lambda$ of $S^\lambda$ on conjugacy class $C_\mu$ given by $\mu=(\mu_1,\cdots,\mu_k)$ with $\mu_1\geqslant\cdots\geqslant \mu_k\geqslant 1$ equals to the coefficient of the monomial $x_1^{\ell_1}\cdots x_n^{\ell_n}$ in polynomial  
> 
> $$\prod_{i=1}^k(x_1^{\mu_i}+\cdots+x_n^{\mu_i})\prod_{i<j}(x_i-x_j),$$
> 
> where $\ell_i=\lambda_i+n-i$.
{ #4b468a}



> [!corollary]
> The dimension of Specht module $S^\lambda$ is
> 
> $$\dim S^\lambda=f^\lambda=\frac{n!}{\ell_1!\cdots\ell_n!}\prod_{1\leqslant i<j\leqslant n}(\ell_i-\ell_j).$$

`\begin{proof}`
Note that $\dim S^\lambda=\chi^\lambda(1)$, then by [[MATH/代数专题/Nodes/10.6 Frobenius Character Formula#^4b468a\|#^4b468a]] 

$$\dim S^\lambda=\mbox{ coefficient of }x_1^{\ell_1}\cdots x_n^{\ell_n}\mbox{ in } (x_1+\cdots+x_n)^n\prod_{1\leqslant i<j\leqslant n}(x_i-x_j).$$

By Vandermonde determinant, 

$$\sum_{\sigma\in S^n}\mathrm{sgn}\sigma \cdot x_1^{n-\sigma(1)}x_2^{n-\sigma(2)-1}\cdots x_n^{n-\sigma(n)}=\det \left|\begin{matrix} x_1^{n-1} & x_2^{n-1} & \cdots & x_n^{n-1} \\
\vdots & \vdots &  & \vdots \\ 
x_1 & x_2 & \cdots & x_n \\
1 & 1 & \cdots & 1\end{matrix}\right|=\prod_{1\leqslant i< j\leqslant n}(x_i-x_j)$$

and so the coefficient of $x_1^{\ell_1}\cdots x_n^{\ell_n}$ in

$$(x_1+\cdots+x_n)^n\prod_{1\leqslant i<j\leqslant n}(x_i-x_j)=\left(\sum_{k_1+\cdots+k_n=n}\frac{n!}{k_1!\cdots k_n!}x_1^{k_1}\cdots x_n^{k_n}\right)\left(\sum_{\sigma\in S^n}\mathrm{sgn}\sigma \cdot x_1^{n-\sigma(1)}x_2^{n-\sigma(2)-1}\cdots x_n^{n-\sigma(n)}\right)$$

is 

$$\sum_{\sigma\in S_n}\mathrm{sgn}\sigma\frac{n!}{(\ell_1-n+\sigma(1))!\cdots(\ell_n-n+\sigma(n))!}=n!\det\left|\begin{matrix}
\dfrac{1}{(\ell_1-n+1)!} & \cdots & \dfrac{1}{(\ell_n-n+1)!} \\
\vdots  &  & \vdots \\
\dfrac{1}{\ell_1!} & \cdots & \dfrac{1}{\ell_n!}
\end{matrix}\right|=\frac{n!}{\ell_1!\cdots\ell_n!}\prod_{1\leqslant i<j\leqslant n}(\ell_i-\ell_j).$$

Now we finish the proof.
`\end{proof}`


# Hook Length Formula

For a Young tableau $\lambda$ and the element on $i$ th row, $j$ th column, define $h(i,j)=\lambda_i+\lambda_j'-i-j+1$, where $\lambda_j'$ is the number of $j$ th column. 

The hook length formula tells us that

$$\dim S^\lambda=f^\lambda=\frac{n!}{\prod_{(i,j)\in\lambda}h(i,j)}.$$

[[Pasted image 20241202154117.png|Here]] is an example, and [[MATH/代数专题/Nodes/List 4 (Oral Exam)#^xmv91w\|here]] is a proof.

# Young-Fibonacci Lattice

The number of standard tableaux for $\lambda$ is the number of path from $\emptyset$ to $\lambda$ diagram in Young diagram. Here is an example. 

![Pasted image 20241204154913.png|300](/img/user/%E9%99%84%E4%BB%B6/Pasted%20image%2020241204154913.png). 