---
{"dg-publish":true,"permalink":"/MATH/代数专题/Nodes/10.9 Characteristical Map/","dgPassFrontmatter":true}
---


For a finite group $G$, its irreducible characters form basis for the space of class functions $F_c(G,\mathbb{C})$. Define $R_n=F_c(S_n,\mathbb{C})$ and $R=\oplus_{n\geqslant 0}R_n$ with $R_0=\mathbb{C}$. 

We introduce on the $R$ product. For any $\phi\in R_n$ and $\psi\in R_m$, where $\phi$ (rep. $\psi$) is a character of $S_n$ (rep. $S_m$), define $\phi\cdot\psi\in R_{n+m}$ as 

$$\phi\cdot \psi=(\phi\otimes \psi)\uparrow_{Sn\times S_m}^{S_{n+m}}.$$

> [!theorem]
> The product $\cdot$ on $R$ is commutative and associative.

`\begin{proof}`
Define $\rho=\left(\begin{array}{ccc}1 & \cdots & n & n+1 & \cdots & m\\ m+1& \cdots & n+m & 1 & \cdots & m\end{array}\right)$. Then there is a bijection 

$$S_n\times S_m\to S_m\times S_n,\omega\mapsto \rho^{-1}\omega\rho.$$

For associativity, use $\left(W\uparrow_K
{ #H}
\right)\uparrow_H^G=W \uparrow_K^G$.
`\end{proof}`


Furthermore, we can equip the algebra $R$ with an inner product

$$
\left\langle f, g\right\rangle=\sum_{n \geqslant 0}\left\langle f_n,g_n\right\rangle _{S_n}.
$$

> [!definition]
> Define the character map 
> 
> $$\mathrm{ch}:R\to \Lambda,f\mapsto \frac{1}{n!}\sum_{\omega\in S_n}f(\omega)p_\omega.$$
> 

**Remark.** For any $f\in R_n$ and any conjugacy class $C_\mathscr p$ with representative $\mathscr p$, we can write the character map as

$$\mathrm{ch}:f\to \frac{1}{n!}\sum_{\mathscr p\vdash n}f(C_p)p_{\mathscr p}|C_{\mathscr p}|=\sum_{\mathscr p\vdash n}z_{\mathcal p}^{-1}f(C_\mathscr p)p_\mathscr p.$$

> [!theorem]
> The characteristic map $\mathrm{ch}:R\to \Lambda$ is an isometry and an algebra isomorphism. Moreover, $\mathrm{ch}(\chi^\lambda)=\mathscr s_\lambda$ and $\mathrm{ch}(\phi^\lambda)=h_{\lambda}$, where $\phi^\lambda$ is the character of permutation module $M^\lambda$.
{ #492b55}


`\begin{proof}`

> [!NOTE] A Generalization
> Let $G$ be a finite group, and let $A$ be an associative algebra. If $\Phi,\Psi:G\to A$ are functions, we may define a bilinear form with values in $A$ 
> 
> $$\left\langle\Phi,\Psi\right\rangle =\frac{1}{|G|}\sum_{g\in G}\Phi(g)\Psi(g^{-1}).$$
> 
> If $\Phi$ is a class function on $H$ and $\Psi$ is a class function on $G$, the generalized [[MATH/代数专题/Nodes/9 Frobenius Reciprocity\|Frobenius reciprocity]] still holds, that is 
> 
> $$\left\langle \Phi\uparrow^G,\Psi\right\rangle =\left\langle \Phi,\Psi\downarrow_H\right\rangle$$
> 
> where $\Phi\downarrow_H(h)=\Phi(h)$ and $\Psi\uparrow
{ #G}
(g)=\frac{1}{|H|}\sum_{x\in G}\Psi(x^{-1}gx)$ with the convention that $\Psi(g')=0$ if $g'\notin H$. 

For any $f,g\in R_n$, there is

$$\begin{aligned}
\left\langle \mathrm{ch}(f),\mathrm{ch}(g)\right\rangle &=\left\langle \sum_{\mathscr p\vdash n}z_{\mathscr p}^{-1}f(C_{\mathscr p})p_{\mathscr p},\sum_{\lambda\vdash n}z_{\lambda}^{-1}g(C_\lambda)p_\lambda\right\rangle \\
&=\sum_{\lambda\vdash n}z_{\lambda}^{-1}z_{\lambda}^{-1}f(C_\lambda)g(C_\lambda)z_{\lambda}\\
&=\sum_{\lambda\vdash n}|C_\lambda|\frac{1}{n!}f(C_\lambda)g(C_\lambda)\\
&=\left\langle f,g\right\rangle 
\end{aligned}$$

Also note that $g(\omega^{-1})=g(\omega)$. 

Since $p_\omega=p_{\omega^{-1}}$ for $\omega\in S_n$ and $\mathrm{ch}(f)=\left\langle f,p\right\rangle$, we have

$$\begin{aligned}
\mathrm{ch}(fg)&=\left\langle fg,p\right\rangle=\left\langle(f\otimes g)\uparrow_{S_n\times S_m}^{S_{m\times n}},p\right\rangle\\
&=\frac{1}{n!m!}\sum_{\sigma\in S_n,\tau\in S_m}(f\otimes g)(\sigma\tau)p_{\sigma\tau}\\
&=\frac{1}{n!m!}\sum_{(\sigma,\tau)\in S_n\times S_m}f(\sigma)g(\tau)p_\sigma p_\tau\\
&=\left(\frac{1}{n!}\sum_{\sigma\in S_n}f(\sigma)p_\sigma\right)\left(\frac{1}{m!}\sum_{\tau\in S_m}g(\tau)p_\tau\right)\\
&=\mathrm{ch}(f)\mathrm{ch}(g)
\end{aligned}$$

and so $\mathrm{ch}$ is a homomorphism.

Let $\eta_n$ be the trivial representation of $S_n$, then 

$$\mathrm{ch}(\eta_n)=\left\langle \eta_n,p\right\rangle=\sum_{\lambda\vdash n}z_{\lambda}^{-1}p_\lambda=h_\lambda.$$

Recall that the permutation module $M^\lambda=1\uparrow_{S_\lambda}^{S_n}$ with $S_\lambda=S_{\lambda_1}\times\cdots\times S_{\lambda_k}$. Then $\phi^\lambda=\eta_{\lambda_1}\cdots\eta_{\lambda_k}$ yields that 

$$\mathrm{ch}(\phi^\lambda)=\mathrm{ch}(\eta_{\lambda_1})\cdots\mathrm{ch}(\eta_{\lambda_k})=h_{\lambda_1}\cdots h_{\lambda_k}=h_\lambda.$$

To prove that $\mathrm{ch}(\chi^\lambda)=\mathscr s_\lambda$, note that

$$\widetilde {\chi^\lambda}=\left|\begin{matrix}
\eta_{\lambda_1} & \cdots & \eta_{\lambda_1+m-1} \\
\vdots &  & \vdots \\
\eta_{\lambda_m-m+1} & \cdots & \eta_{\lambda_m}
\end{matrix}\right|$$

and $\mathrm{ch}(\widetilde {\chi^\lambda})=\mathscr s_\lambda$. Now we finish the proof, as $\widetilde {\chi^\lambda}$ is induced $\chi^\lambda$. 
`\end{proof}`


> [!corollary]
> The character table $\chi_{\mathscr p}^\lambda$ is the transition matrix between bases $p_\lambda$ and $\mathscr s_\lambda$ of $\Lambda^n$.
{ #7ed3d1}


`\begin{proof}`
It suffices to show $p_{\mathscr p}=\sum_{\lambda}\chi_{\mathscr p}^\lambda \mathscr s_\lambda$. By [[MATH/代数专题/Nodes/10.9 Characteristical Map#^492b55\|#^492b55]] we have 

$$\mathscr s_\lambda=\mathrm{ch}(\chi^\lambda)=\sum_{\mathscr p}z_{\mathscr p}^{-1}\chi_{\mathscr p}^\lambda p_{\mathscr p}$$

and so $\chi_{\mathscr p}^\lambda=\left\langle \mathscr s_\lambda, p_\mathscr p\right\rangle$. It deduces that 

$$\left\langle \mathscr s_\lambda,p_\mu\right\rangle =\sum_{\mathscr p} z_\mathscr p^{-1}\chi_{\mathscr p}^{\lambda}\left\langle p_\mathscr p,p_\mu\right\rangle =z_{\mu}^{-1}\chi_{\mu}^\lambda z_{\mu}=\chi_{\mu}^\lambda.$$

Now we finish the proof.
`\end{proof}`


> [!corollary] Frobenius character formula 
> If $\rho=(\rho_1,\cdots,\rho_m)$ with $\rho_1\geqslant \rho_2\geqslant\cdots\geqslant \rho_m\geqslant 1$, then for any $k\geqslant\ell(\lambda)$ the value $\chi_\rho^\lambda$ is the coefficient of $x_1^{\ell_1}\cdots x_k^{\ell_k}$ in the monomial 
> 
> $$\prod_{i=1}^m(x_1^{\rho_i}+\cdots+x_k^{\rho_i})\prod_{1\leqslant i< j\leqslant k}(x_i-x_j)$$
> 
> where $\ell_i=\lambda_i+k-i$ for $i=1,\cdots,k$. 

**Remark.** It has been proved in [[MATH/代数专题/Nodes/10.6 Frobenius Character Formula#^4b468a\|10.6 Frobenius Character Formula#^4b468a]].

`\begin{proof}`
Recall that $p_{\rho}=\prod_{i=1}^m(x_1^{\rho_i}+\cdots+x_k^{\rho_i})$ and 


<div class="transclusion internal-embed is-loaded"><a class="markdown-embed-link" href="/math//nodes/10-8-symmetric-polynomials/#i6y60w" aria-label="Open link"><svg xmlns="http://www.w3.org/2000/svg" width="24" height="24" viewBox="0 0 24 24" fill="none" stroke="currentColor" stroke-width="2" stroke-linecap="round" stroke-linejoin="round" class="svg-icon lucide-link"><path d="M10 13a5 5 0 0 0 7.54.54l3-3a5 5 0 0 0-7.07-7.07l-1.72 1.71"></path><path d="M14 11a5 5 0 0 0-7.54-.54l-3 3a5 5 0 0 0 7.07 7.07l1.71-1.71"></path></svg></a><div class="markdown-embed">



> [!definition]
> Suppose $\lambda=(\lambda_1,\cdots,\lambda_m)$ is a partition of $n$ of length at most $m$. The Schur polynomial $\mathscr s_\lambda$ is defined by 
> 
> $\mathscr s_\lambda=\frac{\left|\begin{matrix}
x_1^{\lambda_1+m-1} & \cdots  & x_m^{\lambda_1+m-1} \\
x_1^{\lambda_2+m-2} & \cdots & x_m^{\lambda_2+m-2} \\
\vdots &  & \vdots \\
x_1^{\lambda_m} & \cdots & x_m^{\lambda_m}
\end{matrix}\right|}{\left|\begin{matrix}
x_1^{m-1} & \cdots  & x_m^{m-1} \\
x_1^{m-2} & \cdots & x_m^{m-2} \\
\vdots &  & \vdots \\
1 & \cdots & 1
\end{matrix}\right|}.$
> 
> 

</div></div>


By [[MATH/代数专题/Nodes/10.9 Characteristical Map#^7ed3d1\|#^7ed3d1]], we have $p_{\mathscr p}=\sum_{\lambda}\chi_{\mathscr p}^\lambda \mathscr s_\lambda$ and it deduces that 

$$\mathrm{LHS}=\sum_{\mu}\chi_{\rho}^\mu\left|\begin{matrix}
x_1^{\mu_1+k-1} & ... & x_k^{\mu_1+k-1} \\
\vdots &  & \vdots \\
x_1^{\mu_l} & \cdots & x_k^{\mu_k}
\end{matrix}\right|.$$

Therefore, the coefficient of $x_1^{\ell_1}\cdots x_k^{\ell_k}$ with $\ell_i=\lambda_i+k-i$ of right hand side is $\chi_{\rho}^\lambda$. 
`\end{proof}`