---
{"dg-publish":true,"permalink":"/MATH/抽象代数III/Nodes/2 250304/","dgPassFrontmatter":true}
---


# Category

> [!definition]
> A category $\mathcal D$ is called a subcategory of a category $\mathcal C$ if
> - the objects of $\mathcal D$ is a subclass of the objects of $\mathcal C$
> - for any objects $A,B$ of $\mathcal D$, one has that 
> 	- $\mathrm{Hom}_{\mathcal D}(A,B)\subseteq\mathrm{Hom}_{\mathcal C}(A,B)$;
> 	- $1_A$ and the product of morphisms for $\mathcal D$ is the same as for $\mathcal C$. 
> 
> The subcategory $\mathcal D$ is called *full* if $\mathrm{Hom}_{\mathcal D}(A,B)=\mathrm{Hom}_{\mathcal C}(A,B)$.

> [!definition]
> Let $\mathcal C$ be a category. Define $\mathcal C^{\mathrm{op}}$ as
> - objects of $\mathcal{C}^{\mathrm{op}}$ are the objects of $\mathcal{C}$
> - $\mathrm{Hom}_{\mathcal{C}^{\mathrm{op}}}(A,B)=\mathrm{Hom}_{\mathcal{C}^{\mathrm{op}}}(B,A)$
> 
> satisfying that
> - if $f\in \mathrm{Hom}_{\mathcal{C}^\mathrm{op}}(A,B)$ and $g\in \mathrm{Hom}_{\mathcal{C}^\mathrm{op}}(B,C)$, then $gf$ in $\mathcal{C}^\mathrm{op}$ equals $fg$ in $\mathcal{C}$; and
> - $1_{\mathcal{C}^\mathrm{op}}=1_{\mathcal{C}}$.

> [!definition]
> Let $\mathcal{C}$ and $\mathcal{D}$ be two categories. A *covariant functor* $F$ form $\mathcal{C}$ to $\mathcal{D}$ satisfies
> - for any object $X\in\mathcal{C}$, $F(X)$ is an object of $\mathcal{D}$;
> - for any $f\in\mathrm{Hom}_{\mathcal{C}}(X,Y)$, $F(f)\in\mathrm{Hom}_{\mathcal{D}}(F(X),F(Y))$ such that
>   
>   $$F(g \circ f)=F(g) \circ F(f) ,\mbox{ for any } f\in\mathrm{Hom}_{\mathcal{C}}(X,Y),g\in\mathrm{Hom}_{\mathcal{C}}(Y,Z)\tag{*}$$
> 
> - $F(\mathrm{id}_X)=\mathrm{id}_{F(X)}$.
> 
> If $(*)$ is modified to
> 
> $$F(g \circ f)=F(f) \circ F(g) ,\mbox{ for any } f\in\mathrm{Hom}_{\mathcal{C}}(X,Y),g\in\mathrm{Hom}_{\mathcal{C}}(Y,Z)$$
> 
> then $F:\mathcal{C}\to \mathcal{D}$ is called a *contravariant functor*. In particular, a contravariant functor from $\mathcal C$ to $\mathcal{D}$ is a covariant functor from $\mathcal{C}^\mathrm{op}$ to $\mathcal{D}$. 

**Remark.** In general, if $R$ is non-commutative, $\mathrm{Hom}_R(M,N)$ is not an $R$-module. Notice that 

$$(r_1r_2)f(m)=f(r_1r_2m)=(r_1f)(r_2m)=(r_2r_1f)(m)$$

and $r_1r_2,r_2r_1$ are not always equal.

**Examples.** 
- Given $R$-module $M$, define
  
  $$\begin{aligned}\mathrm{Hom}_R(M,\cdot):R\mbox{-module}&\to \mbox{Ab},\\N&\mapsto\mathrm{Hom}_R(M,N),\\f&\mapsto h_f:t\mapsto f\circ t.\end{aligned}$$
  
  We can verify that $\mathrm{Hom}_R(M,\cdot)$ is a covariant functor. 
- Similarly, given $R$-module $M$, define 
  
  $$\begin{aligned}\mathrm{Hom}_R(\cdot, M):R\mbox{-module}&\to \mathrm{Ab},\\N&\mapsto\mathrm{Hom}(N,M),\\f&\mapsto h_f:t\mapsto t\circ f\end{aligned}$$
  
  We can verify that $\mathrm{Hom}_R(\cdot, M)$ is a contravariant functor.



# Bimodule

## Hom Functor

> [!definition]
> Let $R$ and $S$ be rings with identity. An abelian group $M$ is a *left $R$- right $S$-bimodule* in case $M$ is both a left $R$-module and a right $S$-module for which the two scalar multiplication jointly satisfy $r(xs)=(rx)s$ for any $r\in R,x\in M,s\in S$. 

**Remark.** Here are some notations:
- ${}_RM$: $M$ is a left $R$-module
- $M_R$: $M$ is a right $R$-module
- ${}_{R}M_S$: $M$ is a left $R$- right $S$-bimodule.

Let $U:={}_RU_S$ be a bimodule. Then for any $R$-module ${}_RM$, 
- $\mathrm{Hom}_R(U,M)$ is a left $S$-module. 
	- For any $f\in\mathrm{Hom}_R(U,M)$, define $(sf)(u)=f(us)$. 
	- $\mathrm{Hom}_R(U,\cdot):R\mbox{-module}\to S\mbox{-module}$ is a covariant functor; 
- $\mathrm{Hom}_R(M,U)$ is a right module-$S$. 
	- For any $g\in\mathrm{Hom}_R(M,U)$, define $(gs)(m)=g(m)s$.
	- $\mathrm{Hom}_R(\cdot,U):R\mbox{-module}\to \mbox{module-}S$ is a contravariant functor. See [[MATH/交换代数/Nodes/2 Modules#^jj28ws\|2 Modules#^jj28ws]]. 

## Tensor Functor

Suppose $M={}_SM_R$ and $N={}_RN$ are two modules, then $M\otimes _RN$ is a $S$-module. Similarly, suppose $M=M_R$ and $N={}_RN_T$ are two modules, then $M\otimes_RN$ is a module-$T$. 

If ${}_SM_R$ and ${}_RN_T$ are bimodules, then $M\otimes_R N$ is a left $S$- right $T$-bimodule with $s(m\otimes n)=(sm)\otimes n$ and $(m\otimes n)t=m\otimes(nt)$. 

> [!proposition]
> Given a bimodule ${}_SU_R$, define 
> 
> $$U\otimes_R\cdot:R\mbox{-module}\to S\mbox{-module}, M\mapsto U\otimes_RM,f\mapsto \mathrm{id} _U\otimes f$$
> 
> and it is a covariant functor.
> 
> Similarly, define 
> 
> $$\cdot\otimes_RR:\mbox{module-}S\to \mbox{module-}R, M\mapsto M\otimes_RU,f\mapsto f\otimes\mathrm{id} _U$$
> 
> and it is also a covariant functor.


# Exact Sequence and Exact Functors


> [!definition]
> Let $F:R\mbox{-module}\to S\mbox{-module}$ be a covariant functor. 
> - We say $F$ is *left exact* if for any exact sequence $0\to N\stackrel{\varphi}{\to}M\stackrel{\psi}{\to}P$, the sequence $0\to F(N)\stackrel{F(\varphi)}{\to}F(M)\stackrel{F(\psi)}{\to}F(P)$ is exact. 
> - We say $F$ is *right exact* if for any exact sequence $N\stackrel{\varphi}{\to}M\stackrel{\psi}{\to}P\to 0$, the sequence $F(N)\stackrel{F(\varphi)}{\to}F(M)\stackrel{F(\psi)}{\to}F(P)\to 0$ is exact.

> [!definition]
> A contravariant $G:R\mbox{-module}\to\rm{Ab}$ is called left (rep. right) exact if it is a left (rep. right) exact as a covariant functor $(R\mbox{-module})^\mathrm{op}\to\rm{Ab}$. 

> [!definition]
> A functor is called *exact* if it is both left exact and right exact.



<div class="transclusion internal-embed is-loaded"><a class="markdown-embed-link" href="/math//nodes/2-modules/#jj28ws" aria-label="Open link"><svg xmlns="http://www.w3.org/2000/svg" width="24" height="24" viewBox="0 0 24 24" fill="none" stroke="currentColor" stroke-width="2" stroke-linecap="round" stroke-linejoin="round" class="svg-icon lucide-link"><path d="M10 13a5 5 0 0 0 7.54.54l3-3a5 5 0 0 0-7.07-7.07l-1.72 1.71"></path><path d="M14 11a5 5 0 0 0-7.54-.54l-3 3a5 5 0 0 0 7.07 7.07l1.71-1.71"></path></svg></a><div class="markdown-embed">



> [!proposition]
> - Let $M'\stackrel{u}{\to}M\stackrel{ v}{\to}M''\to 0$ $(*)$ be a sequence of $A$-module homomorphism. Then it is exact iff for any $A$-module $N$, the induced sequence
>   
>   $0\to \mathrm{Hom}(M'',N)\stackrel{\overline{v}}{\to}\mathrm{Hom}(M,N)\stackrel{\overline{u}}{\to}\mathrm{Hom}(M',N)\tag{**}$
>   
>   is exact, where $\overline v:f\mapsto f\circ v$ and $\overline u:g\mapsto g\circ u$. 
> - (dual statement) Let $0\to N'\stackrel{u}{\to} N\stackrel{v}{\to} N''(☺️)$ be a sequence. It is exact iff for any $A$-module $M$, the induced sequence 
>   
>   $0\to \mathrm{Hom}(M,N')\stackrel{\overline u}{\to} \mathrm{Hom}(M,N)\stackrel{\overline v}{\to} \mathrm{Hom}(M,N'')\tag{☺️☺️}$
>   
>   is exact. 

</div></div>



> [!theorem]
>  Let ${}_SU_R$ be a bimodule. The functor $U\otimes_R\cdot:R\mbox{-module}\to S\mbox{-module}$ is right exact. 

`\begin{proof}`
![Pasted image 20250316235524.png|500](/img/user/%E9%99%84%E4%BB%B6/Pasted%20image%2020250316235524.png)

Theorem 7.4 is same as [[MATH/抽象代数III/Nodes/1 250218, 250225#^80axob\|1 250218, 250225#^80axob]]. 
`\end{proof}`


# Projective, Injective and Flat Modules

> [!definition]
> Let $M$ be an $R$-module. 
> - $M$ is called *projective* $R$-module if $\mathrm{Hom}_R(M,\cdot)$ is exact.
> - $M$ is called *injective* $R$-module if $\mathrm{Hom}_R(\cdot, M)$ is exact.
> - $M$ is called flat $R$-module if $M\otimes_R\cdot$ is exact.


> [!theorem]
> The following statements about a left $R$-module $P$ are equivalent.
> - Whenever there is an $R$-epimorphism $M\stackrel{g}{\to}N$, and an $R$-homomorphism $P\stackrel{\gamma}{\to}N$, there exists an $R$-homomorphism $\overline\gamma:P\to M$ such that $\gamma=g\overline\gamma$.
> - For each epimorphism $f:{_R}M\to{}_RN$, the map $\mathrm{Hom}_R(P,M)\to\mathrm{Hom}_R(P,N)$ is an epimorphism.
> - For each bimodule structure ${}_RP_S$, the functor $\mathrm{Hom}_R(P,\cdot):R\mbox{-module}\to S\mbox{-module}$ is exact.
> - For every exact sequence $M\stackrel{f'}{\to}M\stackrel{g}{\to}M''$ in $R$-module, the sequence $\mathrm{Hom}_R(P,M')\stackrel{\mathrm{Hom}_R(P,f)}{\to}\mathrm{Hom}_R(P,M)\stackrel{\mathrm{Hom}_R(P,g)}{\to}\mathrm{Hom}_R(P,M'')$ is exact. 
{ #9f21f9}


`\begin{proof}`
Not too hard.
`\end{proof}`


> [!theorem]
> The following statements about a (left) $R$-module $P$ are equivalent:
> - $P$ is projective.
> - Every epimorphism $M\stackrel{f}{\to}P$ splits, that is, there exists $R$-homomorphism $g:P\to M$ such that $fg=1_P$.
> - $P$ is isomorphic to a direct summand of a free left $R$-module.
{ #3rkmd6}


`\begin{proof}`
i) -> ii) By [[MATH/抽象代数III/Nodes/2 250304#^9f21f9\|#^9f21f9]] i), take $\gamma=\mathrm{id}_P:P\to P$. 

ii)->iii) Note that every module is a quotient of free modules, then by [[MATH/抽象代数II/Nodes/2.2 Modules#^qtklfv\|2.2 Modules#^qtklfv]] we finish the proof.

iii)->i) Assume that $P\oplus Q=F$ is a free $R$-module. Note that the free module $F=\oplus_{i\in I}R$ is projective as $\mathrm{Hom}_R(F,M)=\prod_{i\in I}M$ and the functor $M\mapsto\prod_{i\in I}M$ is exact. Then $\mathrm{Hom}_R(F,\cdot)=\mathrm{Hom}_R(P,\cdot)\times\mathrm{Hom}_R(Q,\cdot)$ as functors, hence both $P$ and $Q$ are projective.
`\end{proof}`


> [!theorem] Schanuel's lemma
> Let $R$ be a ring with identity. If $0 \rightarrow K \rightarrow P \rightarrow M \rightarrow 0$ and $0 \rightarrow K^{\prime} \rightarrow P^{\prime} \rightarrow M \rightarrow 0$ are short exact sequences of $R$-modules and $P$ and $P^{\prime}$ are projective, then $K \oplus P^{\prime}$ is isomorphic to $K^{\prime} \oplus P$.

`\begin{proof}`
Define the following submodule of $P \oplus P^{\prime}$, where $\phi: P \rightarrow M$ and $\phi^{\prime}: P^{\prime} \rightarrow M$ 

$$X=\left\{(p, q) \in P \oplus P^{\prime}: \phi(p)=\phi^{\prime}(q)\right\}.$$

The map $\pi: X \rightarrow P$, where $\pi$ is defined as the projection of the first coordinate of $X$ into $P$, is surjective. Since $\phi^{\prime}$ is surjective, for any $p \in P$, one may find a $q \in P^{\prime}$ such that $\phi(p)=\phi^{\prime}(q)$. This gives $(p, q) \in X$ with $\pi(p, q)=p$. Now the kernel of the map $\pi$ is

$$\begin{aligned}\operatorname{ker} \pi & =\{(0, q):(0, q) \in X\} \\
& =\left\{(0, q): \phi^{\prime}(q)=0\right\} \\
& \cong \operatorname{ker} \phi^{\prime} \cong K^{\prime}.
\end{aligned}$$

We may conclude that there is a short exact sequence

$$0 \rightarrow K^{\prime} \rightarrow X \rightarrow P \rightarrow 0.$$

Since $P$ is projective and this sequence splits, so $X \cong K^{\prime} \oplus P$ by [[MATH/抽象代数III/Nodes/2 250304#^3rkmd6\|#^3rkmd6]]. Similarly, we can write another map $\pi^{\prime}: X \rightarrow P^{\prime}$, and the same argument as above shows that there is another short exact sequence

$$
0 \rightarrow K \rightarrow X \rightarrow P^{\prime} \rightarrow 0
$$

and so $X \cong P^{\prime} \oplus K$. Combining the two equivalences for $X$ gives the desired result.
`\end{proof}`
