---
{"dg-publish":true,"permalink":"/MATH/抽象代数III/Nodes/6 250401/","dgPassFrontmatter":true}
---


> [!proposition]
> Let $A$ be an Artinian ring, and let $U$ be a finitely generated $A$-module. 
> - TFAE for an $A$-submodule of $U$:
> 	- $V=\mathrm{Rad}U$
> 	- $V$ is the smallest submodule of $U$ with semisimple quotient. 
> 	- $J(A)U=V$
> - TFAE for an $A$-submodule of $U$:
> 	- $V=\mathrm{soc} U$
> 	- $V$ is the largest semisimple submodule of $U$
> 	- $V=\{u\in U:J(A)u=0\}$.

`\begin{proof}`
(1) Let $V=J(A)U$. Then $U/V$ is an $A/J(A)$-module, which is semisimple. On the other hand, if $V'\subseteq U$ with semisimple quotient $U/V'$, then $J(A)(U/V')=0$ and $J(A)U\subseteq V'$.

(2) Notice that $\{u\in U:J(A)u=0\}$ is the largest submodule of $U$ annihilated by $J(A)$. So it is an $A/J(A)$-module and so it is semisimple. For the largest, each simple module is annihilated by $J(A)$. 

> [!definition]
> Let $U$ be a finitely generated $A$-module with $A$ Artinian. Define inductively $\mathrm{Rad}^n(U)=\mathrm{Rad}(\mathrm{Rad}^{n-1}(U))$ and $\mathrm{soc}^n(U)/\mathrm{soc}^{n-1}(U)=\mathrm{soc}(U/\mathrm{soc}^{n-1}(U))$.
> 
> So $\mathrm{Rad}^n(U)=J(A)^nU$, $\mathrm{soc}^n(U)=\{u\in U:J(A)^nu=0\}$. 


Chains of submodules:
- $\mathrm{Rad}^0(U)\supseteq \mathrm{Rad}(U)\supseteq\cdots$ is called radical series/Lowey series.
- $0\subseteq \mathrm{soc}(U)\subseteq\mathrm{soc}^2(U)\subseteq\cdots$ is called socle series. 

We call $\mathrm{Rad}^{n-1}U/\mathrm{Rad}^{n}U$ radical layer/Lowey layer; $\mathrm{soc}^n(U)/\mathrm{soc}^{n-1}(U)$ socle layer.

> [!lemma]
> $\mathrm{Rad}^n(U\oplus V)=\mathrm{Rad}^n(U)\oplus \mathrm{Rad}^n(V)$.
> $\mathrm{soc}^n(U\oplus V)=\mathrm{soc}^n(U)\oplus \mathrm{soc}^n(V)$.

> [!theorem]
> Let $A$ be an Artinian ring. Let $U$ be an finitely generated $A$-module. The radical series of $U$ is the fastest descending series of submodules of $U$ with semisimple quotient, and the socle series of $U$ is the fastest ascending series with semisimple quotient. 
> 
> The two series terminate and if $m$ and $n$ are the minimal integer with $\mathrm{Rad}^mU=0$ and $\mathrm{soc}^nU=U$, then $m=n$.

`\begin{proof}`
Suppose that $\cdots\subseteq U_2\subseteq U_1\subseteq U_0=U$ is a series of submodules of $U$ with semisimple quotient. We show by induction on $r$ such that $\mathrm{Rad}^r(U)\subseteq U_r$. We prove it by induction. When $r=0$, it is trivial. Now assume that $\mathrm{Rad}^{r-1}(U)\subseteq U_{r-1}$. Then we have 

$$\mathrm{Rad}^{r-1}(U)/(\mathrm{Rad}^{r-1}(U)\cap U_r)\simeq \mathrm{Rad}^{r-1}(U)+U_r/U_r\subseteq U_{r-1}/U_r$$

is semisimple and so $\mathrm{Rad}^{r-1}(U)\cap U_r\supseteq \mathrm{Rad}(\mathrm{Rad}^{r-1}(U))=\mathrm{Rad}^r(U)$. 

Similarly, we can prove the case of socle.

然后不知道他在说什么：
$J(A)^r=0$ for some $r$
$\mathrm{Rad}^r(U)=J(A)^rU=0$
$\mathrm{soc}^r(U)=\{u\in U:J(A)^ru=0\}=U$

长度一样就是比大小两次夹住

`\end{proof}`


> [!lemma]
> - Let $A$ be a semisimple ring, then $A$ is Artinian iff it is Noetherian. 
> - If $A$ is Artinian ring, then it is Noetherian. 

`\begin{proof}`
i) is easy.

ii) $J=J(A)$, $J^2=J\cdot J=\mathrm{Rad}(J)$. consider left $A$-module ${}_A A$, then $J^{n+1}=\mathrm{Rad}(J^n)$. $J^n/J^{n+1}$ is semisimple. To show $A$ is Noetherian, as $A/J$ is Noetherian, it suffices to show $J$ is Noetherian. As $J/J^2$ is Noetherian, it suffices to show $J^2$ is Noetherian. Repeat this procedure, and finitely it suffices to show $J^r=0$ is Noetherian. Now we finish the proof. 



$$A\supseteq J\supseteq\cdots \supseteq  J^r=0$$

`\end{proof}`


> [!definition]
> Let $I$ be a $2$-sided ideal of $R$. $f$ is an idempotent of $R$. $e=f+I$ is an idempotent in $R/I$. We say $f$ lifts $e$. 

If for every idempotent $e$ of $R/I$ there is an idempotent $f\in R$ lifting $e$, then we say we can lift idempotents from $R/I$ to $R$. 

> [!theorem]
> Let $I$ be a nilpotent ideal of $R$, then we can lift idempotent from $R/I$ to $R$. That is, for every idempotent $e$ of $R/I$, there is an idempotent $f\in R$ with $e=f+I$. If $e$ is primitive, so is any lift $f$. 

`\begin{proof}`
We define inductively idempotent $e_i\in R/I_i$ such that $e_i+I^{i-1}/I^i=e_{i-1}$ for each $i$ and $e_1=e$. Suppose $e_{i-1}$ is an idempotent of $R/I^{i-1}$. Pick any element $a\in R/I^i$ with $a+I^{i-1}=e_{i-1}$, then $a^2-a\in I^{i-1}/I^i$. Note that $a^2-a=0\in R/I^i$. 

Put $e_i=3a^2-2a^3$, then $e_i+I_{i-1}=e_{i-1}$, and 

$$e_i^2-e_i=-(3-2a)(1+2a)(a^2-a)^2=0$$

in $R/I^i$. If $I^r=0$, then $f=e_r$ is what we desired. 

Suppose $e$ is primitive and $f$ has an idempotent decomposition $f=f_1+f_2$ Then $e=e_1+e_2$ with $f_i+I=e_i$. Since $e$ is primitive, one of $e_1,e_2$ is $0$ and so WLOG $f_1+I=0$ and so $f_1\in I$. It contradicts with $f_1$ idempotent. 
`\end{proof}`


> [!corollary]
> Let $I$ be a nilpotent ($2$-sided) ideal of a ring $R$ and let $1=e_1+\cdots+e_n$ be an idempotent decomposition in $R/I$. Then we have an idempotent decomposition $1=f_1+\cdots+f_n$ in $R$ with $e_i=f_i+I$. If $e_i$ are primitive, so are $f_i$. 

`\begin{proof}`
Induction on $n$. $n=1$ is trivial, and now we assume it holds for $m<n$. 

Write $1=e_1+E$ in $R/I$ if $e_2+\cdots+e_n=E$. Note that $E$ is an idempotent and it is orthogonal to $e_1$. Then we lift $e_1$ to $f_1\in R$, that is, $e_1=f_1+I$. In $R$, $1=f_1+F$ where $F=1-f_1$, then $F$ lifts $E$. 

$F$ is the identity of the ring $FRF$, and $FIF$ is a nilpotent ideal of $FRF$. Consider the composition homomorphism 

$$FRF\hookrightarrow R\twoheadrightarrow R/I$$

whose kernel is $FRF\cap I=FIF$, because
- $FIF\subseteq FRF\cap I$ 
- for any $x\in FRF\cap I$, $FxF\subseteq FIF$. 

We get an inclusion $FRF/FIF\hookrightarrow R/I$, and its image is $E(R/I)E$. Note that $E(R/I)E$ has identity $E$. By induction hypothesis, $F=f_2+\cdots+f_n$ with $f_i+I=e_i$ for $i\geqslant 2$. Thus $1=f_1+\cdots+f_n$ and we finish the proof.
`\end{proof}`


> [!corollary]
> Let $f$ be an idempotent in a ring $R$ that has a nilpotent ideal $I$. Then $f$ is primitive in $R$ iff $f+I$ is primitive in $R/I$. 

`\begin{proof}`
One direction is easy. 

Assume that $f$ is imprimitive, then consider the ring $fRf$, whose identity is $f$. 
`\end{proof}`


> [!lemma]
> Let $A$ be a semisimple Artinian ring. 
> - There is a primitive idempotent decomposition $1=e_1+\cdots+e_n$. This corresponds $A=Ae_1\oplus\cdots\oplus Ae_n$ where $Ae_i$ is simple. 
> - For every simple $A$-module $S$, there is a primitive idempotent $e$ with $S\simeq Ae$.
> - for any simple $A$-module $S$, there exists $1\leqslant i\leqslant n$, $e_iS\neq 0$ and if $T$ is simple $A$-module with $T\not\simeq S$, then $e_i T=0$. 

 `\begin{proof}`
 iii) $S=1S=(e_1+\cdots+e_n)S$. There exists $i$ such that $e_iS\neq 0$. For simple $A$-module $T$, $e_iT=e_iAe\simeq \mathrm{Hom}_R(Ae,Ae_i)=0$ if $Ae\not\simeq A e_i$,  

> [!theorem]
> Let $A$ be an Artinian ring, and let $S$ be a simple $A$-module. 
> - There is an indecomposable projective $A$-module $P_S$ with $P_S/\mathrm{Rad}(P_S)\simeq S$ of the form $P_S\simeq A_f$ where $f$ is a primitive idempotent in $A$.
> - The idempotent $f$ has the property that $fS\neq 0$, and if $T$ is any simple module with $T\not\simeq S$ then $fT=0$. 
> - $P_S$ is the projective cover of $S$, it is uniquely determined up to isomorphism by $S$. 

`\begin{proof}`
没有听。。。。拍下来了，回头写。
`\end{proof}`

> [!theorem]
> Let $A$ be an Artinian ring. Up to isomorphism, the indecomposable projective $A$-module are exactly the module $P_S$ that are the projective covers of simple modules, and $P_S\simeq P_T$ iff $S\simeq T$. Each $P_S$ appears as direct summand of ${}_A A$ (left regular module) with multiplicity equal to the multiplicity of $S$ as a summand of ${}_{A/J(A)}A/J(A)$. Precisely, ${}_A A\simeq \oplus_S(P_S)^{n_S}$, where $S$ runs through simple $A$-modules up to isomorphism, and $n_S=\dim_D S$ with $D=\mathrm{End}_A(S)$. 

`\begin{proof}`
In $A/J(A)$, $1=e_1+\cdots+e_n$. 
In $A$, $1=f_1+\cdots+f_n$ and ${}_A A=Af_1\oplus\cdots\oplus A f_n$. 

The $Ae_i$ is simple and $Ae_i\simeq Af_i/\mathrm{Rad}(Af_i)$ with $Af_i=P_S$. 

$P/\mathrm{Rad} P\simeq S_1\oplus\cdots\oplus S_t$, then $P\to S_1\oplus\cdots\oplus S_t$ is a projective cover. Also $P_{S_1}\oplus\cdots\oplus P_{S_t}\to S_1\oplus\cdots\oplus S_t$ is a projective cover. So $P\simeq P_{S_1}\oplus\cdots\oplus P_{S_t}$.

![Pasted image 20250401213631.png|500](/img/user/%E9%99%84%E4%BB%B6/Pasted%20image%2020250401213631.png)

`\end{proof}`

> [!theorem]
> Let $A$ be an Artinian ring, and let $U$ be $A$-module. Then $U$ has a projective cover. 

`\begin{proof}`
We only prove for $U$ finitely generated. 

![Pasted image 20250401214707.png|500](/img/user/%E9%99%84%E4%BB%B6/Pasted%20image%2020250401214707.png)

`\end{proof}`

Let $A$ be an Artinian ring. Let $V$ be a finitely generated $A$-module. Then $V$ has a composition series, which is both Artinian and Noetherian. For any simple $A$-module $S$, the number of the composition factors isomorphic to $S$ is called the multiplicity of $S$ in $V$. 

> [!theorem]
> Let $A$ be an Artinian ring, and let $f\in A$ be a primitive idempotent. Assume that $e=f+J(A)\in A/J(A)=\overline A$ is a primitive idempotent. Then the multiplicity of $\overline A e$ in any finitely generated $A$-module $V$ is equal to the composition length of $fV$ as an $fAf$-module. 

`\begin{proof}`
Let $V=V_0\supseteq V_1\supseteq\cdots\supseteq V_n=0$ be a composition series of $V$. Consider $fAf$-modules 

$$fV=fV_0\supseteq\cdots\supseteq fV_n=0$$

where $V_i/V_{i+1}\simeq \overline A e$ iff $f(V_i/V_{i+1})\neq 0$. And in this case, 

$$e\overline Ae\simeq f(V_i/V_{i+1})=fV_i+V_{i+1}/V_{i+1}\simeq fV_i/(V_i\cap V_{i+1})=fV_i/fV_{i+1}$$

which is also simple as $fAf$-module. 
`\end{proof}`

